Moved nat-based literals, etc. to new folder
- Spruced up old proofs in literal, assign, clause
- Moved nat-based literals to src/deprecated
- Renamed X_general to X

src/cnf/assignment.lean
@@ -1,179 +1,233 @@
 /-
-This file expands on the definition for assignment given in literal.lean
-
-Also defines equivalence on domains for assignments.
+Defines the properties of assignments on polymorphic variables,
+including equisatisfiability and equivalence on domains.
 
 Authors: Cayden Codel, Jeremy Avigad, Marijn Heule
 Carnegie Mellon University
 -/
 
+import data.list.basic
 import cnf.literal
 
-import data.list.basic
-import data.list.perm
+universe u
+
+-- Represents the parametric type of the variable stored in the literal
+variables {V : Type u} [decidable_eq V] [inhabited V]
 
 namespace assignment
 
 open literal
 open list
 
-instance : inhabited assignment := ⟨(λ _, tt)⟩
+/-! # Properties -/
 
-/-! # Equivalence on domain definition -/
+instance : inhabited (assignment V) := ⟨(λ _, tt)⟩
 
--- Making the ∀ n ∈ l into ∀ {n : nat}, n ∈ l is hard because sometimes the types don't agree
-def eqod (α₁ α₂ : assignment) (l : list nat) : Prop := ∀ n ∈ l, α₁ n = α₂ n
+/-! # Equisatisfiability -/
 
+/- Formulas are functions from assignments to booleans.
+   Two formulas are equisatisfiable if the satisfiability of one
+   implies the satisfiability of the other.
+-/
+def eqsat (f₁ f₂ : assignment V → bool) : Prop := 
+  (∃ (α₁ : assignment V), f₁ α₁ = tt) ↔ (∃ (α₂ : assignment V), f₂ α₂ = tt)
+
+@[refl] theorem eqsat.refl (f : assignment V → bool) : eqsat f f := ⟨id, id⟩
+
+@[symm] theorem eqsat.symm {f₁ f₂ : assignment V → bool} :
+  eqsat f₁ f₂ → eqsat f₂ f₁ :=
+assume h, ⟨λ heq, h.mpr heq, λ heq, h.mp heq⟩
+
+theorem eqsat_comm {f₁ f₂ : assignment V → bool} :
+  (eqsat f₁ f₂) ↔ (eqsat f₂ f₁) :=
+⟨eqsat.symm, eqsat.symm⟩
+
+@[trans] theorem eqsat.trans {f₁ f₂ f₃ : assignment V → bool} :
+  eqsat f₁ f₂ → eqsat f₂ f₃ → eqsat f₁ f₃ :=
+begin
+  intros h₁ h₂,
+  split,
+  { intro h,
+    exact h₂.mp (h₁.mp h) },
+  { intro h,
+    exact h₁.mpr (h₂.mpr h) }
+end
+
+/-! # Equivalence on domain -/
+
+/- Two assignments are equivalent on a domain of variables if they agree
+   on the truth value of that variable for all variables in the list.
+-/
+def eqod (α₁ α₂ : assignment V) (l : list V) : Prop := ∀ v ∈ l, α₁ v = α₂ v
+
+-- Better notation for this?
 notation α₁ ` ≡[`:50 l `]≡ `:50 α₂ := eqod α₁ α₂ l
 
-/-! # Equivalence relation proofs -/
-
-@[refl] theorem eqod.refl (α : assignment) (l : list nat) : α ≡[l]≡ α :=
+@[refl] theorem eqod.refl (α : assignment V) (l : list V) : α ≡[l]≡ α :=
 by simp [eqod]
 
-@[symm] theorem eqod.symm {α₁ α₂ : assignment} {l : list nat} (p : α₁ ≡[l]≡ α₂) :
+@[symm] theorem eqod.symm {α₁ α₂ : assignment V} {l : list V} (p : α₁ ≡[l]≡ α₂) :
   α₂ ≡[l]≡ α₁ :=
-assume n hn, (p n hn).symm
+assume v hv, (p v hv).symm
 
-theorem eqod_comm {α₁ α₂ : assignment} {l : list nat} :
+theorem eqod_comm {α₁ α₂ : assignment V} {l : list V} :
   (α₁ ≡[l]≡ α₂) ↔ (α₂ ≡[l]≡ α₁) :=
 ⟨eqod.symm, eqod.symm⟩
 
-@[trans] theorem eqod.trans {α₁ α₂ α₃ : assignment} {l : list nat} :
+@[trans] theorem eqod.trans {α₁ α₂ α₃ : assignment V} {l : list V} :
   (α₁ ≡[l]≡ α₂) → (α₂ ≡[l]≡ α₃) → (α₁ ≡[l]≡ α₃) :=
-assume h₁ h₂ n hn, eq.trans (h₁ n hn) (h₂ n hn)
+assume h₁ h₂ v hv, eq.trans (h₁ v hv) (h₂ v hv)
 
-/-! # General properties -/
--- Many of these are general list properties, so the proofs are very short
-
-@[simp] theorem eqod_nil (α₁ α₂ : assignment) : α₁ ≡[nil]≡ α₂ :=
+@[simp] theorem eqod_nil (α₁ α₂ : assignment V) : α₁ ≡[nil]≡ α₂ :=
 by simp [eqod]
 
--- This could get its own section? If domains become sets instead of lists, then moot
-theorem eqod_perm {α₁ α₂ : assignment} {l₁ l₂ : list nat} :
+-- If domains become sets instead of lists, then perms become moot
+theorem eqod_perm {α₁ α₂ : assignment V} {l₁ l₂ : list V} :
   l₁ ~ l₂ → (α₁ ≡[l₁]≡ α₂) → α₁ ≡[l₂]≡ α₂ :=
-assume h₁ h₂ n hn, h₂ n ((perm.mem_iff h₁).mpr hn)
+assume h₁ h₂ v hv, h₂ v ((perm.mem_iff h₁).mpr hv)
 
-theorem eqod_of_eqod_cons {α₁ α₂ : assignment} {n : nat} {l : list nat} :
-  (α₁ ≡[n :: l]≡ α₂) → α₁ ≡[l]≡ α₂ :=
+theorem eqod_of_eqod_cons {α₁ α₂ : assignment V} {v : V} {l : list V} :
+  (α₁ ≡[v :: l]≡ α₂) → α₁ ≡[l]≡ α₂ :=
 by simp [eqod]
 
--- If two assignments agree on a value outside the domain, it can be extended
-theorem eqod_cons_of_eq_of_not_mem_of_eqod {α₁ α₂ : assignment} {n : nat} {l : list nat} :
-  (α₁ ≡[l]≡ α₂) → n ∉ l → α₁ n = α₂ n → α₁ ≡[n :: l]≡ α₂ :=
+-- From the set point of view, we might want non-membership of new value v
+theorem eqod_cons_of_eq_of_not_mem_of_eqod {α₁ α₂ : assignment V} {v : V} {l : list V} :
+  (α₁ ≡[l]≡ α₂) → α₁ v = α₂ v → α₁ ≡[v :: l]≡ α₂ :=
 begin
-  intros h₁ hnm heq m hm,
+  intros h₁ heq m hm,
   rcases eq_or_mem_of_mem_cons hm with rfl | hml,
   { exact heq },
   { exact h₁ m hml }
 end
 
-theorem eqod_subset_of_eqod {α₁ α₂ : assignment} {l₁ l₂ : list nat} :
+theorem eqod_subset_of_eqod {α₁ α₂ : assignment V} {l₁ l₂ : list V} :
   l₁ ⊆ l₂ → (α₁ ≡[l₂]≡ α₂) → α₁ ≡[l₁]≡ α₂ :=
-assume h₁ h₂ n hn, h₂ n (h₁ hn)
+assume h₁ h₂ v hv, h₂ v (h₁ hv)
 
-theorem eqod_union_of_eqod {α₁ α₂ : assignment} {l₁ l₂ : list nat} :
-  (α₁ ≡[l₁]≡ α₂) → (α₁ ≡[l₂]≡ α₂) → α₁ ≡[l₁ ∪ l₂]≡ α₂ :=
-assume h₁ h₂ n hn, by { cases (mem_union.mp hn), exact h₁ n h, exact h₂ n h }
+-- The types of mem_union don't check?
+--theorem eqod_union_of_eqod [decidable_eq V] [has_union (list V)] [has_mem V (list V)] {α₁ α₂ : assignment V} {l₁ l₂ : list V} :
+--  (α₁ ≡[l₁]≡ α₂) → (α₁ ≡[l₂]≡ α₂) → α₁ ≡[l₁ ∪ l₂]≡ α₂ :=
+--assume h₁ h₂ v hv, by { cases (mem_union.mp hn), exact h₁ n h, exact h₂ n h }
 
-theorem eqod_inter_of_eqod {α₁ α₂ : assignment} {l₁ l₂ : list nat} :
-  (α₁ ≡[l₁]≡ α₂) → (α₁ ≡[l₂]≡ α₂) → α₁ ≡[l₁ ∩ l₂]≡ α₂ :=
-assume h₁ _ n hn, h₁ n (mem_inter.mp hn).1
+-- Same thing here, with mem_inter
+--theorem eqod_inter_of_eqod [has_inter (list V)] {α₁ α₂ : assignment V} {l₁ l₂ : list V} :
+--  (α₁ ≡[l₁]≡ α₂) → (α₁ ≡[l₂]≡ α₂) → α₁ ≡[l₁ ∩ l₂]≡ α₂ :=
+--assume h₁ _ v hv, h₁ v (mem_inter.mp hv).1
 
-theorem eqod_append_left {α₁ α₂ : assignment} {l₁ l₂ : list nat} :
+theorem eqod_append_left {α₁ α₂ : assignment V} {l₁ l₂ : list V} :
   (α₁ ≡[l₁ ++ l₂]≡ α₂) → α₁ ≡[l₁]≡ α₂ :=
 assume h, eqod_subset_of_eqod (sublist.subset (sublist_append_left l₁ l₂)) h
 
-theorem eqod_append_right {α₁ α₂ : assignment} {l₁ l₂ : list nat} :
+theorem eqod_append_right {α₁ α₂ : assignment V} {l₁ l₂ : list V} :
   (α₁ ≡[l₁ ++ l₂]≡ α₂) → α₁ ≡[l₂]≡ α₂ :=
 assume h, eqod_subset_of_eqod (sublist.subset (sublist_append_right l₁ l₂)) h
 
 /-! # Evaluation and extension -/
 
-theorem eval_eq_of_mem_of_eqod {α₁ α₂ : assignment} {ns : list nat} {l : literal} :
-  (α₁ ≡[ns]≡ α₂) → l.var ∈ ns → literal.eval α₁ l = literal.eval α₂ l :=
-by { cases l; simp only [literal.eval, var]; intros h hl; simp [h l hl] }
+theorem eval_eq_of_mem_of_eqod {α₁ α₂ : assignment V} {l : list V} {lit : literal V} :
+  (α₁ ≡[l]≡ α₂) → lit.var ∈ l → literal.eval α₁ lit = literal.eval α₂ lit :=
+by { cases lit; simp only [literal.eval, var]; intros h hl; simp only [h lit hl] }
 
 -- Sometimes the domain of equivalence needs to be extended according to a particular assignment
-theorem exists_extended_assignment_of_assignment (α₁ : assignment) {l : list nat} {n : nat} :
-  n ∉ l → ∀ (b : bool), ∃ (α₂ : assignment), (α₁ ≡[l]≡ α₂) ∧ α₂ n = b :=
+theorem exists_extended_assignment_of_assignment [decidable_eq V] (α₁ : assignment V) {l : list V} {v : V} :
+  v ∉ l → ∀ (b : bool), ∃ (α₂ : assignment V), (α₁ ≡[l]≡ α₂) ∧ α₂ v = b :=
 begin
-  intros hn b,
-  use (λ x, if x = n then b else α₁ x),
+  intros hv b,
+  use (λ (x : V), if x = v then b else α₁ x),
   simp [eqod],
   intros x hx,
-  simp [ne_of_mem_of_not_mem hx hn]
+  simp [ne_of_mem_of_not_mem hx hv]
 end
 
--- The domain can be extended by whole lists
-theorem exists_list_extended_assignment_of_assignment (α₁ : assignment) {l e : list nat} :
-  disjoint l e → ∀ (f : nat → bool), ∃ (α₂ : assignment), (α₁ ≡[l]≡ α₂) ∧ (∀ n ∈ e, α₂ n = f n) :=
+-- The domain can be extended by whole lists instead
+theorem exists_list_extended_assignment_of_assignment [decidable_eq V] (α₁ : assignment V) {l e : list V} :
+  disjoint l e → ∀ (f : V → bool), ∃ (α₂ : assignment V), (α₁ ≡[l]≡ α₂) ∧ (∀ n ∈ e, α₂ n = f n) :=
 begin
   intros hle f,
   use (λ x, if x ∈ e then f x else α₁ x),
   simp [eqod],
   split,
-  { intros n hn, simp [hle hn] },
+  { intros v hv, simp [hle hv] },
   { intros n ha hb, contradiction }
 end
 
-/-! # Append -/
+/-! # ite -/
+-- A process by which membership of one set uses assignment 1, else assignment 2
 
--- When two domains are disjoint, their combination are equivalent on each respective domain
-def append (α₁ α₂ : assignment) (l₁ l₂ : list nat) (h : disjoint l₁ l₂) :=
-  (λ n, if n ∈ l₁ then α₁ n else α₂ n)
+protected def ite (α₁ α₂ : assignment V) (l : list V) : assignment V :=
+  λ v, if v ∈ l then α₁ v else α₂ v
 
-theorem append_eval_left_of_mem_left (α₁ α₂ : assignment) {l₁ l₂ : list nat} (h : disjoint l₁ l₂) {n : nat} :
-  n ∈ l₁ → (append α₁ α₂ l₁ l₂ h) n = α₁ n :=
+@[simp] theorem ite_nil (α₁ α₂ : assignment V) : 
+  ∀ (v : V), (assignment.ite α₁ α₂ []) v = α₂ v :=
+assume v, by simp [assignment.ite]
+
+theorem ite_pos (α₁ α₂ : assignment V) {l : list V} {v : V} :
+  v ∈ l → (assignment.ite α₁ α₂ l) v = α₁ v :=
+assume h, by simp [assignment.ite, h]
+
+theorem ite_neg (α₁ α₂ : assignment V) {l : list V} {v : V} :
+  v ∉ l → (assignment.ite α₁ α₂ l) v = α₂ v :=
+assume h, by simp [assignment.ite, h]
+
+theorem ite_pos_of_lit (α₁ α₂ : assignment V) {l : list V} {lit : literal V} :
+  lit.var ∈ l → literal.eval (assignment.ite α₁ α₂ l) lit = literal.eval α₁ lit :=
 begin
-  intro hn,
-  simp [append, disjoint_left.mp h hn],
-  intro hf,
-  exact absurd hn hf
+  cases lit,
+  { simp [literal.var, literal.eval], exact ite_pos α₁ α₂ },
+  { simp [literal.var, literal.eval],
+    assume h,
+    rw ite_pos α₁ α₂ h }
 end
 
-theorem append_eval_left_of_not_mem_left (α₁ α₂ : assignment) {l₁ l₂ : list nat} (h : disjoint l₁ l₂) {n : nat} :
-  n ∉ l₁ → (append α₁ α₂ l₁ l₂ h) n = α₂ n :=
+theorem ite_neg_of_lit (α₁ α₂ : assignment V) {l : list V} {lit : literal V} :
+  lit.var ∉ l → literal.eval (assignment.ite α₁ α₂ l) lit = literal.eval α₂ lit :=
 begin
-  intro h,
-  simp [append, h]
+  cases lit,
+  { simp [literal.var, literal.eval], exact ite_neg α₁ α₂ },
+  { simp [literal.var, literal.eval],
+    assume h,
+    rw ite_neg α₁ α₂ h }
 end
 
-theorem append_eval_right_of_mem_right (α₁ α₂ : assignment) {l₁ l₂ : list nat} (h : disjoint l₁ l₂) {n : nat} :
-  n ∈ l₂ → (append α₁ α₂ l₁ l₂ h) n = α₂ n :=
-begin
-  intro hn,
-  simp [append, disjoint_right.mp h hn]
-end
+theorem eqod_ite_of_disjoint (α₁ α₂ : assignment V) {l₁ l₂ : list V} :
+  disjoint l₁ l₂ → α₂ ≡[l₂]≡ (assignment.ite α₁ α₂ l₁) :=
+assume h v hv, by simp [assignment.ite, disjoint_right.mp h hv]
 
-theorem eqod_of_append_left (α₁ α₂ : assignment) {l₁ l₂ : list nat} (h : disjoint l₁ l₂) :
-  (append α₁ α₂ l₁ l₂ h) ≡[l₁]≡ α₁ :=
-assume n hn, append_eval_left_of_mem_left α₁ α₂ h hn
-
-theorem eqod_of_append_right (α₁ α₂ : assignment) {l₁ l₂ : list nat} (h : disjoint l₁ l₂) :
-  (append α₁ α₂ l₁ l₂ h) ≡[l₂]≡ α₂ :=
-assume n hn, append_eval_right_of_mem_right α₁ α₂ h hn
+theorem eqod_ite_of_subset (α₁ α₂ : assignment V) {l₁ l₂ : list V} :
+  l₂ ⊆ l₁ → α₁ ≡[l₂]≡ (assignment.ite α₁ α₂ l₁) :=
+assume h v hv, by simp [assignment.ite, h hv]
 
 /-! # Miscellaneous -/
 
 -- Constant function assignments
-def all_tt : assignment := (λ _, tt)
-def all_ff : assignment := (λ _, ff)
+def all_tt : assignment V := (λ _, tt)
+def all_ff : assignment V := (λ _, ff)
 
-theorem all_tt_eval_tt : ∀ (n : nat), all_tt n = tt := by simp [all_tt]
-theorem all_ff_eval_ff : ∀ (n : nat), all_ff n = ff := by simp [all_ff]
+theorem all_tt_eval_tt : ∀ (n : V), all_tt n = tt := by simp [all_tt]
+theorem all_ff_eval_ff : ∀ (n : V), all_ff n = ff := by simp [all_ff]
 
 -- There may be times where setting or flipping variables is important
-def set_var (α : assignment) (n : nat) (b : bool) : assignment :=
-  λ x, if x = n then b else α x
+def set_var [decidable_eq V] (α : assignment V) (v : V) (b : bool) : assignment V :=
+  λ x, if x = v then b else α x
 
-def flip_var (α : assignment) (n : nat) : assignment :=
-  λ x, if x = n then bnot (α n) else α x
+def flip_var [decidable_eq V] (α : assignment V) (v : V) : assignment V :=
+  λ x, if x = v then bnot (α v) else α x
 
-theorem eval_eq_of_set_var {α : assignment} {n : nat} {b : bool} : (set_var α n b) n = b :=
+theorem eval_eq_of_set_var {α : assignment V} {v : V} {b : bool} : 
+  (set_var α v b) v = b :=
 by simp [set_var]
 
-theorem eval_ne_of_flip_var {α : assignment} {n : nat} : α n = bnot ((flip_var α n) n) :=
+theorem eval_ne_of_flip_var {α : assignment V} {v : V} :
+  α v = bnot ((flip_var α v) v) :=
 by simp [flip_var]
+
+theorem eqod_set_var_of_not_mem (α : assignment V) (v : V) (b : bool) :
+  ∀ (l : list V), v ∉ l → (α ≡[l]≡ (set_var α v b)) :=
+begin
+  intros l h,
+  unfold set_var,
+  intros z hz,
+  simp [ne_of_mem_of_not_mem hz h]
+end
 
 end assignment
