src/cnf/clause.lean
@@ -1,6 +1,7 @@
 /-
-This file contains the definition of a Boolean (disjunctive) clause (as in CNF).
-This particular implementation has clauses as lists.
+This file contains the definition of a Boolean (disjunctive) clause.
+This particular implementation has clauses as lists, although a set definition
+is sufficient as well.
 
 Authors: Cayden Codel, Jeremy Avigad, Marijn Heule
 Carnegie Mellon Univeristy
@@ -9,130 +10,135 @@ Carnegie Mellon Univeristy
 import cnf.literal
 import cnf.assignment
 import basic
+
 import data.nat.basic
 import init.data.nat.lemmas
 import data.list.basic
 import data.list.count
 import data.list.nodup
 import data.list.perm
-
-import data.finset.basic
 import init.logic
+import init.function
 
-/- (Disjunctive) clauses are lists of literals, joined by logical ORs. -/
-def clause := list literal
+universe u
+
+-- Represents the parametric type of the variable stored in the literal
+variables {V : Type u} [decidable_eq V] [inhabited V]
+
+/- Disjunctive clauses are lists of literals, joined by logical ORs. -/
+def clause (V : Type u) := list (literal V)
+
+-- Note that the above definition allows for duplication of literals, whereas
+-- a set definition would not. Lists also allow for computable functions,
+-- while Lean sets are noncomputable by default
 
 namespace clause
 
+open function
 open literal
 open list
 
-/-! # Properties, borrowed from lists -/
+/-! # Properties -/
 
-instance : inhabited clause := ⟨[default literal]⟩
+-- Many of these properties follow directly from lists
 
-instance has_decidable_eq [s : decidable_eq literal] : decidable_eq clause
+instance : inhabited (clause V) := ⟨[default (literal V)]⟩
+
+instance has_decidable_eq : decidable_eq (clause V)
 | []        []        := is_true rfl
 | (a :: as) []        := is_false (λ h, list.no_confusion h)
 | []        (b :: bs) := is_false (λ h, list.no_confusion h)
 | (a :: as) (b :: bs) :=
-  match s a b with
+  match (literal.decidable_eq V) a b with
   | is_true hab  :=
     match has_decidable_eq as bs with
-    | is_true habs  := is_true (eq.subst hab (eq.subst habs rfl))
-    | is_false nabs := is_false (λ h, list.no_confusion h (λ _ habs, absurd habs nabs))
+    | is_true h := is_true (eq.subst hab (eq.subst h rfl))
+    | is_false hf := is_false (λ h, list.no_confusion h (λ _ ha, absurd ha hf))
     end
-  | is_false nab := is_false (λ h, list.no_confusion h (λ hab _, absurd hab nab))
+  | is_false hf := is_false (λ h, list.no_confusion h (λ hab _, absurd hab hf))
   end
 
-instance : has_mem literal clause := ⟨list.mem⟩
-instance : has_emptyc clause := ⟨list.nil⟩ -- Refactor empty into [] below?
-instance : has_union clause := ⟨list.union⟩
-instance : has_inter clause := ⟨list.inter⟩
-instance : has_singleton literal clause := ⟨λ l, [l]⟩ 
-instance : has_insert literal clause := ⟨list.insert⟩
-instance : has_append clause := ⟨list.append⟩
-instance : has_subset clause := ⟨list.subset⟩
+instance : has_mem (literal V) (clause V) := ⟨list.mem⟩
+instance : has_emptyc (clause V) := ⟨list.nil⟩ -- Refactor empty into [] below?
+instance : has_union (clause V) := ⟨list.union⟩
+instance : has_inter (clause V) := ⟨list.inter⟩
+instance : has_singleton (literal V) (clause V) := ⟨λ l, [l]⟩ 
+instance : has_insert (literal V) (clause V) := ⟨list.insert⟩
+instance : has_append (clause V) := ⟨list.append⟩
+instance : has_subset (clause V) := ⟨list.subset⟩
 
-/-! # Evaluation under assignment -/
+instance (l : literal V) (c : clause V) : decidable (l ∈ c) :=
+by apply_instance
 
-/- The clause represents a disjunction, so we evaluate literals until tt is found -/
-protected def eval (α : assignment) (c : clause) : bool :=
+/-! # eval -/
+
+-- Note: protected b/c many constructs will have an evaluation def
+/- To evaluate the clause, fold false along until a true evaluation is found -/
+protected def eval (α : assignment V) (c : clause V) : bool :=
   c.foldr (λ l b, b || (l.eval α)) ff
 
 -- Proving properties of the fold operation
-lemma eval_op_left_comm (α : assignment) : 
-  left_commutative (λ (l : literal) (b : bool), b || (literal.eval α l)) :=
+lemma eval_op_left_comm (α : assignment V) : 
+  left_commutative (λ (l : literal V) (b : bool), b || (l.eval α)) :=
 assume l₁ l₂ b, by simp [bool.bor_comm, bool.bor_assoc]
 
-@[simp] theorem eval_nil (α : assignment) : clause.eval α [] = ff := rfl
+@[simp] theorem eval_nil (α : assignment V) : clause.eval α [] = ff := rfl
 
-@[simp] theorem eval_singleton (α : assignment) (l : literal) : clause.eval α [l] = literal.eval α l :=
-by simp [clause.eval]
+@[simp] theorem eval_singleton (α : assignment V) (l : literal V) : 
+  clause.eval α [l] = l.eval α :=
+by simp only [clause.eval, foldr, ff_bor]
 
-theorem eval_cons (α : assignment) (l : literal) (c : clause) : 
+theorem eval_cons (α : assignment V) (l : literal V) (c : clause V) : 
   clause.eval α (l :: c) = (literal.eval α l) || (clause.eval α c) :=
-by simp [clause.eval, bool.bor_comm]
+by simp only [clause.eval, foldr, bool.bor_comm]
 
-theorem ne_nil_of_eval_tt {α : assignment} {c : clause} : clause.eval α c = tt → c ≠ [] :=
-by { contrapose, simp, intro h, simp [h] }
-
-lemma exists_literal_eval_tt_of_eval_tt {α : assignment} {c : clause} :
-  clause.eval α c = tt → ∃ l ∈ c, literal.eval α l = tt :=
-begin
-  induction c with l ls ih,
-  { contradiction },
-  { intro h,
-    simp [eval_cons] at h,
-    cases h,
-    { use [l, h] },
-    { rcases ih h with ⟨l₂, hl, he⟩,
-      use [l₂, mem_cons_of_mem l hl, he] } }
-end
-
-lemma eval_tt_of_exists_literal_eval_tt {α : assignment} {c : clause} :
-  (∃ l ∈ c, literal.eval α l = tt) → clause.eval α c = tt :=
-begin
-  rintros ⟨l, hl, he⟩,
-  induction c with d ds ih,
-  { exact absurd hl (not_mem_nil _) },
-  { rcases eq_or_ne_mem_of_mem hl with rfl | ⟨hne, hds⟩,
-    { simp [eval_cons, he] },
-    { simp [eval_cons, ih hds] } }
-end
-
-theorem eval_tt_iff_exists_literal_eval_tt {α : assignment} {c : clause} : 
+theorem eval_tt_iff_exists_literal_eval_tt {α : assignment V} {c : clause V} : 
   clause.eval α c = tt ↔ ∃ l ∈ c, literal.eval α l = tt :=
-⟨exists_literal_eval_tt_of_eval_tt, eval_tt_of_exists_literal_eval_tt⟩
-
-lemma forall_literal_eval_ff_of_mem_of_eval_ff {α : assignment} {c : clause} :
-  clause.eval α c = ff → ∀ l ∈ c, literal.eval α l = ff :=
 begin
-  induction c with d ds ih,
-  { simp },
-  { simp [eval_cons],
-    intros hl hds,
-    exact and.intro hl (ih hds) }
+  split,
+  { induction c with l ls ih,
+    { contradiction },
+    { simp [eval_cons],
+      intro h, cases h,
+      { use [l, h] },
+      { rcases ih h with ⟨l₂, hl, he⟩,
+        use [l₂, mem_cons_of_mem l hl, he] } } },
+  { rintros ⟨l, hl, he⟩,
+    induction c with d ds ih,
+    { exact absurd hl (not_mem_nil _) },
+    { rcases eq_or_ne_mem_of_mem hl with rfl | ⟨hne, hds⟩,
+      { simp [eval_cons, he] },
+      { simp [eval_cons, ih hds] } } }
 end
 
-lemma eval_ff_of_forall_literal_eval_ff {α : assignment} {c : clause} :
-  (∀ l ∈ c, literal.eval α l = ff) → clause.eval α c = ff :=
+theorem ne_nil_of_eval_tt {α : assignment V} {c : clause V} :
+  c.eval α = tt → c ≠ [] :=
 begin
-  induction c with l ls ih,
-  { simp },
-  { intro h,
-    simp [eval_cons, h l (mem_cons_self l ls)],
-    have : ∀ (m : literal), m ∈ ls → literal.eval α m = ff,
-    { intros m hm, exact h m (mem_cons_of_mem l hm) },
-    exact ih this }
+  intro h,
+  rcases eval_tt_iff_exists_literal_eval_tt.mp h with ⟨l, hmem, _⟩,
+  exact ne_nil_of_mem hmem
 end
 
-theorem eval_ff_iff_forall_literal_eval_ff {α : assignment} {c : clause} : 
+theorem eval_ff_iff_forall_literal_eval_ff {α : assignment V} {c : clause V} : 
   clause.eval α c = ff ↔ ∀ l ∈ c, literal.eval α l = ff :=
-⟨forall_literal_eval_ff_of_mem_of_eval_ff, eval_ff_of_forall_literal_eval_ff⟩
+begin
+  split,
+  { induction c with l ls ih,
+    { simp },
+    { simp [eval_cons],
+      intros hl hds,
+      exact and.intro hl (ih hds) } },
+  { induction c with l ls ih,
+    { simp },
+    { intro h,
+      simp [eval_cons, h l (mem_cons_self l ls)],
+      have : ∀ (m : literal V), m ∈ ls → literal.eval α m = ff,
+      { intros m hm, exact h m (mem_cons_of_mem l hm) },
+      exact ih this } }
+end
 
-theorem eval_tautology {c : clause} {l : literal} : 
-  l ∈ c → l.flip ∈ c → ∀ (α : assignment), clause.eval α c = tt :=
+theorem eval_tautology {c : clause V} {l : literal V} : 
+  l ∈ c → l.flip ∈ c → ∀ (α : assignment V), clause.eval α c = tt :=
 begin
   intros hl hlf α,
   apply eval_tt_iff_exists_literal_eval_tt.mpr,
@@ -141,12 +147,9 @@ begin
   { use [l, hl, h] }
 end
 
--- From a set POV, similarity becomes moot
-theorem eval_sim (α : assignment) {c₁ c₂ : clause} : c₁ ~ c₂ → clause.eval α c₁ = clause.eval α c₂ :=
-assume h, perm.foldr_eq (eval_op_left_comm α) h ff
+-- Evaluation of subsets and sublists tie in to evaluation nicely
 
--- More set-like properties for evaluation
-theorem eval_tt_of_subset_eval_tt {α : assignment} {c₁ c₂ : clause} :
+theorem eval_tt_of_subset_eval_tt {α : assignment V} {c₁ c₂ : clause V} :
   c₁ ⊆ c₂ → clause.eval α c₁ = tt → clause.eval α c₂ = tt :=
 begin
   intros h₁ h₂,
@@ -155,7 +158,7 @@ begin
   use [l, h₁ hl, he]
 end
 
-theorem eval_ff_of_superset_eval_ff {α : assignment} {c₁ c₂ : clause} :
+theorem eval_ff_of_superset_eval_ff {α : assignment V} {c₁ c₂ : clause V} :
   c₁ ⊆ c₂ → clause.eval α c₂ = ff → clause.eval α c₁ = ff :=
 begin
   intros h₁ h₂,
@@ -165,698 +168,598 @@ begin
   exact h₂ l (h₁ hl)
 end
 
-theorem eval_tt_of_sublist_eval_tt {α : assignment} {c₁ c₂ : clause} :
+theorem eval_tt_of_sublist_eval_tt {α : assignment V} {c₁ c₂ : clause V} :
   c₁ <+ c₂ → clause.eval α c₁ = tt → clause.eval α c₂ = tt :=
 assume h₁, eval_tt_of_subset_eval_tt (sublist.subset h₁)
 
-theorem eval_ff_of_superlist_eval_ff {α : assignment} {c₁ c₂ : clause} :
+theorem eval_ff_of_superlist_eval_ff {α : assignment V} {c₁ c₂ : clause V} :
   c₁ <+ c₂ → clause.eval α c₂ = ff → clause.eval α c₁ = ff :=
 assume h₁, eval_ff_of_superset_eval_ff (sublist.subset h₁)
 
-theorem eval_tt_cons_of_eval_tt {α : assignment} {c : clause} (l : literal) :
+theorem eval_tt_cons_of_eval_tt 
+  {α : assignment V} {c : clause V} (l : literal V) :
   clause.eval α c = tt → clause.eval α (l :: c) = tt :=
 assume h, eval_tt_of_sublist_eval_tt (sublist_cons l c) h
 
-theorem eval_ff_of_eval_ff_cons {α : assignment} {c : clause} {l : literal} :
+theorem eval_ff_of_eval_ff_cons 
+  {α : assignment V} {c : clause V} {l : literal V} :
   clause.eval α (l :: c) = ff → clause.eval α c = ff :=
 assume h, eval_ff_of_superlist_eval_ff (sublist_cons l c) h
 
-/-! # Falsify and truthify -/
-
--- For any list of natural numbers and assignment, a false clause can be computed
-def falsify : assignment → list nat → clause
-| α []        := []
-| α (n :: ns) := if α n then Neg n :: falsify α ns else Pos n :: falsify α ns
-
--- And here's a companion function that might have fewer uses
--- NOTE: The empty case doesn't work, but the empty case is trivial anyways...
-def truthify : assignment → list nat → clause
-| α []        := []
-| α (n :: ns) := if α n then Pos n :: truthify α ns else Neg n :: truthify α ns
-
-@[simp] lemma falsify_nil (α : assignment) : falsify α [] = [] := rfl
-@[simp] lemma truthify_nil (α : assignment) : truthify α [] = [] := rfl
-
-theorem falsify_eval_ff (α : assignment) (l : list nat) : clause.eval α (falsify α l) = ff :=
-begin
-  induction l with n ns ih,
-  { simp },
-  { cases h : (α n);
-    { simp [falsify, h, eval_cons, literal.eval, ih] } }
-end
-
-theorem truthify_eval_tt (α : assignment) {l : list nat} (hl : l ≠ []) : 
-  clause.eval α (truthify α l) = tt :=
-begin
-  induction l with n ms ih,
-  { contradiction },
-  { cases h : (α n);
-    { simp [truthify, h, literal.eval, eval_cons] } }
-end
-
--- Get rid of these next two?
-theorem map_var_falsify_eq_list (α : assignment) (l : list nat) : map var (falsify α l) = l :=
-begin
-  induction l with n ns ih,
-  { simp },
-  { cases h : (α n);
-    { simp [falsify, h, ih, var] } }
-end
-
-theorem map_var_truthify_eq_list (α : assignment) (l : list nat) : map var (truthify α l) = l :=
-begin
-  induction l with n ns ih,
-  { simp },
-  { cases h : (α n);
-    { simp [truthify, h, ih, var] } }
-end
-
-theorem flip_truthify_eq_falsify (α : assignment) (l : list nat) : 
-  map flip (truthify α l) = falsify α l :=
-begin
-  induction l with n ns ih,
-  { simp },
-  { cases h : (α n);
-    { simp [h, literal.eval, ih, literal.flip, truthify, falsify] } }
-end
-
 /-! ### Counting -/
 
-/- Counts the number of literals that evaluate to true in the clause, under some assignment -/
-def count_tt (α : assignment) (c : clause) : nat :=
-  c.countp (λ l, literal.eval α l = tt)
+/- Counts the number of literals that evaluate to true in the clause, under α -/
+def count_tt (α : assignment V) (c : clause V) : nat :=
+  c.countp (literal.is_true α)
 
-/- Counts the number of literals that evaluate to false in the clause, under some assignment -/
-def count_ff (α : assignment) (c : clause) : nat :=
-  c.countp (λ l, literal.eval α l = ff)
+/- Counts the number of literals that evaluate to false in the clause, under α -/
+def count_ff (α : assignment V) (c : clause V) : nat :=
+  c.countp (literal.is_false α)
 
 /- Counts the number of positive literals in the clause -/
-def count_pos (c : clause) : nat :=
-  c.countp (λ l, is_pos l = tt)
+def count_pos (c : clause V) : nat :=
+  c.countp literal.is_pos
 
 /- Counts the number of negative literals in the clause -/
-def count_neg (c : clause) : nat :=
-  c.countp (λ l, is_neg l = tt)
+def count_neg (c : clause V) : nat :=
+  c.countp literal.is_neg
 
-@[simp] lemma count_tt_nil (α : assignment) : count_tt α [] = 0 := by dec_trivial
-@[simp] lemma count_ff_nil (α : assignment) : count_ff α [] = 0 := by dec_trivial
-@[simp] lemma count_pos_nil : count_pos [] = 0 := by dec_trivial
-@[simp] lemma count_neg_nil : count_neg [] = 0 := by dec_trivial
+@[simp] lemma count_tt_nil (α : assignment V) : count_tt α [] = 0 := rfl
+@[simp] lemma count_ff_nil (α : assignment V) : count_ff α [] = 0 := rfl
+@[simp] lemma count_pos_nil : count_pos ([] : clause V) = 0 := rfl
+@[simp] lemma count_neg_nil : count_neg ([] : clause V) = 0 := rfl
 
-@[simp] theorem count_tt_singleton (α : assignment) (l : literal) : 
-  count_tt α [l] = bool.to_nat (literal.eval α l) :=
-by cases h : (literal.eval α l); { simp [h, count_tt, bool.to_nat] }
+@[simp] theorem count_tt_singleton (α : assignment V) (l : literal V) :
+  count_tt α [l] = cond (l.eval α) 1 0 :=
+by cases h : (l.eval α); { simp [h, count_tt, literal.is_true] }
 
-@[simp] theorem count_ff_singleton (α : assignment) (l : literal) :
-  count_ff α [l] = bool.to_nat (!literal.eval α l) :=
-by cases h : (literal.eval α l); { simp [h, count_ff, bool.to_nat] }
+@[simp] theorem count_ff_singleton (α : assignment V) (l : literal V) :
+  count_ff α [l] = cond (l.eval α) 0 1 :=
+by cases h : (l.eval α); { simp [h, count_ff, literal.is_false] }
 
-@[simp] theorem count_pos_singleton (l : literal) : 
-  count_pos [l] = bool.to_nat (is_pos l) :=
-by cases l; simp [count_pos, bool.to_nat, countp, is_pos]
+@[simp] theorem count_pos_singleton (l : literal V) :
+  count_pos [l] = cond l.is_pos 1 0 :=
+by cases l; simp [count_pos, literal.is_pos]
 
-@[simp] theorem count_neg_singleton (l : literal) : 
-  count_neg [l] = bool.to_nat (is_neg l) :=
-by cases l; simp [count_neg, bool.to_nat, countp, is_neg]
+@[simp] theorem count_neg_singleton (l : literal V) :
+  count_neg [l] = cond l.is_neg 1 0 :=
+by cases l; simp [count_neg, literal.is_neg]
 
-theorem count_tt_cons (α : assignment) (l : literal) (c : clause) : 
-  count_tt α (l :: c) = bool.to_nat (literal.eval α l) + count_tt α c :=
-by cases h : (literal.eval α l); { simp [h, bool.to_nat, and_comm, add_comm, count_tt] }
+theorem count_tt_cons (α : assignment V) (l : literal V) (c : clause V) :
+  count_tt α (l :: c) = cond (l.eval α) (1 + c.count_tt α) (c.count_tt α) :=
+by cases h : (literal.eval α l); 
+  { simp [h, literal.is_true, count_tt, add_comm] }
 
-theorem count_ff_cons (α : assignment) (l : literal) (c : clause) : 
-  count_ff α (l :: c) = bool.to_nat (!literal.eval α l) + count_ff α c :=
-by cases h : (literal.eval α l); { simp [h, bool.to_nat, and_comm, add_comm, count_ff] }
+theorem count_ff_cons (α : assignment V) (l : literal V) (c : clause V) :
+  count_ff α (l :: c) = cond (l.eval α) (c.count_ff α) (1 + c.count_ff α) :=
+by cases h : (literal.eval α l);
+  { simp [h, literal.is_false, count_ff, add_comm] }
 
-theorem count_pos_cons (l : literal) (c : clause) : 
-  count_pos (l :: c) = bool.to_nat (is_pos l) + count_pos c :=
-by cases h : (is_pos l); { simp [h, bool.to_nat, add_comm, count_pos] }
+theorem count_pos_cons (l : literal V) (c : clause V) :
+  count_pos (l :: c) = cond l.is_pos (1 + c.count_pos) c.count_pos :=
+by cases l; { simp [count_pos, literal.is_pos, add_comm] }
 
-theorem count_neg_cons (l : literal) (c : clause) : 
-  count_neg (l :: c) = bool.to_nat (is_neg l) + count_neg c :=
-by cases h : (is_neg l); { simp [h, bool.to_nat, add_comm, count_neg] }
+theorem count_neg_cons (l : literal V) (c : clause V) :
+  count_neg (l :: c) = cond l.is_neg (1 + c.count_neg) c.count_neg :=
+by cases l; { simp [count_neg, literal.is_neg, add_comm] }
 
 -- All the above four functions are capped by the length of the clause
-theorem count_tt_le_length (α : assignment) (c : clause) : count_tt α c ≤ length c :=
+theorem count_tt_le_length (α : assignment V) (c : clause V) :
+  c.count_tt α ≤ c.length :=
 by simp only [count_tt, countp_eq_length_filter, length_filter]
 
-theorem count_ff_le_length (α : assignment) (c : clause) : count_ff α c ≤ length c :=
+theorem count_ff_le_length (α : assignment V) (c : clause V) : 
+  c.count_ff α ≤ c.length :=
 by simp only [count_ff, countp_eq_length_filter, length_filter]
 
-theorem count_pos_le_length (c : clause) : count_pos c ≤ length c :=
+theorem count_pos_le_length (c : clause V) : c.count_pos ≤ c.length :=
 by simp only [count_pos, countp_eq_length_filter, length_filter]
 
-theorem count_neg_le_length (c : clause) : count_neg c ≤ length c :=
+theorem count_neg_le_length (c : clause V) : c.count_neg ≤ c.length :=
 by simp only [count_neg, countp_eq_length_filter, length_filter]
 
 -- count_tt and count_ff are complements of each other
--- There's probably an astute nat lemma that cleans this up
-theorem count_tt_eq_length_sub_cont_ff (α : assignment) (c : clause) :
-  count_tt α c = length c - count_ff α c :=
+theorem count_tt_plus_count_ff_eq_length (α : assignment V) (c : clause V) :
+  c.count_tt α + c.count_ff α = c.length :=
 begin
   induction c with l ls ih,
   { simp },
-  { cases h : (literal.eval α l);
-    simp [count_tt_cons, count_ff_cons, h, bool.to_nat, ih, add_comm 1, nat.add_sub_add_right],
-    { rw add_comm ls.length 1,
-      rw nat.add_sub_assoc (count_ff_le_length α ls) 1,
-      rw add_comm } }
+  { cases h : (l.eval α);
+    simp [count_tt_cons, count_ff_cons, h, ← ih],
+    { rw add_assoc,
+      rw add_comm (count_ff α ls) 1 },
+    { rw add_comm (count_tt α ls + count_ff α ls) 1,
+      rw ← add_assoc } }
+end
+
+theorem count_tt_eq_length_sub_count_ff (α : assignment V) (c : clause V) :
+  c.count_tt α = c.length - c.count_ff α :=
+eq_tsub_of_add_eq (count_tt_plus_count_ff_eq_length α c)
+
+theorem count_ff_eq_length_sub_count_tt (α : assignment V) (c : clause V) :
+  c.count_ff α = c.length - c.count_tt α :=
+begin
+  have := count_tt_plus_count_ff_eq_length α c,
+  rw add_comm at this,
+  exact eq_tsub_of_add_eq this
 end
 
 -- count_pos and count_neg are complements of each other
-theorem count_pos_eq_length_sub_count_neg (c : clause) :
-  count_pos c = length c - count_neg c :=
+theorem count_pos_plus_count_neg_eq_length (c : clause V) :
+  c.count_pos + c.count_neg = c.length :=
 begin
   induction c with l ls ih,
   { simp },
   { cases l;
-    simp [ih, count_pos_cons, count_neg_cons, bool.to_nat, is_pos, is_neg],
-    { rw add_comm ls.length 1,
-      rw nat.add_sub_assoc (count_neg_le_length ls) 1 },
-    { simp [add_comm 1] } }
+    simp [count_pos_cons, count_neg_cons, literal.is_pos, literal.is_neg, ← ih],
+    { rw add_comm (count_pos ls + count_neg ls) 1,
+      rw ← add_assoc },
+    { rw add_assoc,
+      rw add_comm 1 } }
 end
 
-lemma count_tt_eq_zero_of_eval_ff {α : assignment} {c : clause} :
-  clause.eval α c = ff → count_tt α c = 0 :=
+theorem count_pos_eq_length_sub_count_neg (c : clause V) :
+  c.count_pos = c.length - c.count_neg :=
+eq_tsub_of_add_eq (count_pos_plus_count_neg_eq_length c)
+
+theorem count_neg_eq_length_sub_count_pos (c : clause V) :
+  c.count_neg = c.length - c.count_pos :=
 begin
-  induction c with l ls ih,
-  { simp },
-  { simp [eval_cons, count_tt_cons],
-    intros hl hls,
-    simp [hl, bool.to_nat, ih hls] }
+  have := count_pos_plus_count_neg_eq_length c,
+  rw add_comm at this,
+  exact eq_tsub_of_add_eq this
 end
 
-lemma eval_ff_of_count_tt_eq_zero {α : assignment} {c : clause} :
-  count_tt α c = 0 → clause.eval α c = ff :=
+-- Note: A good countp lemma may reduce the forward direction
+theorem count_tt_eq_zero_iff_eval_ff {α : assignment V} {c : clause V} :
+  c.eval α = ff ↔ c.count_tt α = 0 :=
 begin
-  induction c with l ls ih,
-  { simp },
-  { simp [eval_cons, count_tt_cons, bool.to_nat, literal.eval],
-    intros hl hls,
-    simp [cond_ff_of_cond_eq_second_of_ne _ one_ne_zero hl, ih hls] }
+  split,
+  { induction c with l ls ih,
+    { simp },
+    { simp [eval_cons, count_tt_cons],
+      intros hl hls,
+      simp [hl, ih hls] } },
+  { induction c with l ls ih,
+    { simp },
+    { simp [eval_cons, count_tt_cons],
+      have : 1 + count_tt α ls ≠ 0,
+      { rw add_comm,
+        rw ← nat.succ_eq_add_one,
+        exact nat.succ_ne_zero _ },
+      intro h,
+      have := ff_of_cond_eq_of_ne_first this h,
+      simp [this] at h,
+      exact and.intro this (ih h) } }
 end
 
-theorem count_tt_eq_zero_iff_eval_ff {α : assignment} {c : clause} :
-  clause.eval α c = ff ↔ count_tt α c = 0 :=
-⟨count_tt_eq_zero_of_eval_ff, eval_ff_of_count_tt_eq_zero⟩
-
-lemma count_tt_gt_zero_of_eval_tt {α : assignment} {c : clause} :
-  clause.eval α c = tt → count_tt α c > 0 :=
+theorem count_tt_eval_tt_iff_gt_zero {α : assignment V} {c : clause V} :
+  c.eval α = tt ↔ count_tt α c > 0 :=
 begin
-  induction c with l ls ih,
-  { simp },
-  { cases h : (literal.eval α l);
-    simp [h, eval_cons, count_tt_cons, bool.to_nat],
-    { intro hls, exact ih hls },
-    { exact nat.zero_lt_one_add _ } }
+  split,
+  { intro h,
+    apply (countp_pos _).mpr,
+    use eval_tt_iff_exists_literal_eval_tt.mp h },
+  { intro h,
+    apply eval_tt_iff_exists_literal_eval_tt.mpr,
+    use (countp_pos _).mp h } 
 end
 
-lemma eval_tt_of_count_tt_gt_zero {α : assignment} {c : clause} :
-  0 < count_tt α c → clause.eval α c = tt :=
-by { simp only [count_tt, countp_pos, eval_tt_iff_exists_literal_eval_tt], exact id }
+/-! # falsify and truthify -/
 
-theorem count_tt_gt_zero_iff_eval_tt {α : assignment} {c : clause} :
-  clause.eval α c = tt ↔ count_tt α c > 0 :=
-⟨count_tt_gt_zero_of_eval_tt, eval_tt_of_count_tt_gt_zero⟩
+-- For any assignment and variables, there is a false clause on those variables
+-- Simply map each variable in the list to the literal which evaluates to false
+def falsify (α : assignment V) (l : list V) : clause V :=
+l.map (λ v, cond (α v) (Neg v) (Pos v))
 
-theorem count_tt_falsify (α : assignment) (l : list nat) : count_tt α (falsify α l) = 0 :=
+-- For any assignment and variables, there is a true clause on those variables
+-- Note: there is no such clause for the empty set of variables
+def truthify (α : assignment V) (l : list V) : clause V :=
+l.map (λ v, cond (α v) (Pos v) (Neg v))
+
+@[simp] lemma falsify_nil (α : assignment V) : falsify α [] = [] := rfl
+@[simp] lemma truthify_nil (α : assignment V) : truthify α [] = [] := rfl
+
+@[simp] lemma falsify_singleton (α : assignment V) (v : V) :
+  falsify α [v] = cond (α v) [Neg v] [Pos v] :=
+by cases h : α v; { simp [h, falsify] }
+
+@[simp] lemma truthify_singleton (α : assignment V) (v : V) :
+  truthify α [v] = cond (α v) [Pos v] [Neg v] :=
+by cases h : α v; { simp [h, truthify] }
+
+theorem falsify_cons (α : assignment V) (v : V) (vs : list V) :
+  falsify α (v :: vs) = cond (α v) (Neg v :: falsify α vs)
+                                   (Pos v :: falsify α vs) :=
+by cases h : α v; { simp [falsify, map_cons, h] }
+
+theorem truthify_cons (α : assignment V) (v : V) (vs : list V) :
+  truthify α (v :: vs) = cond (α v) (Pos v :: truthify α vs)
+                                    (Neg v :: truthify α vs) :=
+by cases h : α v; { simp [truthify, map_cons, h] }
+
+theorem falsify_eval_ff (α : assignment V) (l : list V) :
+  clause.eval α (falsify α l) = ff :=
+begin
+  induction l with v vs ih,
+  { rw falsify_nil, rw eval_nil },
+  { cases h : (α v);
+    { simp [falsify_cons, h, eval_cons, literal.eval, ih] } }
+end
+
+theorem truthify_eval_tt (α : assignment V) {l : list V} (hl : l ≠ []) : 
+  clause.eval α (truthify α l) = tt :=
+begin
+  induction l with v vs ih,
+  { contradiction },
+  { cases h : (α v);
+    { simp [truthify_cons, h, literal.eval, eval_cons] } }
+end
+
+theorem flip_truthify_eq_falsify (α : assignment V) (l : list V) : 
+  map literal.flip (truthify α l) = falsify α l :=
+begin
+  induction l with v vs ih,
+  { simp },
+  { cases h : (α v);
+    { simp [h, literal.eval, ih, literal.flip, truthify_cons, falsify_cons] } }
+end
+
+theorem count_tt_falsify (α : assignment V) (l : list V) :
+  count_tt α (falsify α l) = 0 :=
 count_tt_eq_zero_iff_eval_ff.mp (falsify_eval_ff α l)
 
-lemma count_tt_truthify (α : assignment) (c : clause) : count_tt α (truthify α (map var c)) = length c :=
+lemma count_tt_truthify (α : assignment V) (l : list V) :
+  count_tt α (truthify α l) = length l :=
 begin
-  induction c with l ls ih,
+  induction l with v vs ih,
   { simp },
-  { cases l; { cases h : (α l);
-    { simp [truthify, h, var, count_tt_cons, bool.to_nat, literal.eval, ih, add_comm] } } }
+  { cases h : α v;
+    { simp [truthify_cons, count_tt_cons, literal.eval, h, ih, add_comm] } }
 end
 
 -- Falsify negates those literals that, if positive, are true
-theorem count_tt_pos_eq_count_neg_falsify (α : assignment) (ns : list nat) : 
-  count_tt α (map Pos ns) = count_neg (falsify α ns) :=
+theorem count_tt_pos_eq_count_neg_falsify (α : assignment V) (l : list V) :
+  count_tt α (map Pos l) = count_neg (falsify α l) :=
 begin
-  induction ns with m ms ih,
+  induction l with v vs ih,
   { simp },
-  { cases h : (α m);
-    { simp [count_tt_cons, h, falsify, count_neg_cons, literal.eval, is_neg, bool.to_nat, ih] } }
+  { cases h : (α v);
+    { simp [map_cons, count_tt_cons, falsify_cons, count_neg_cons, 
+        literal.eval, h, ih, literal.is_neg] } }
 end
 
 -- Sublist theorems (can have subset theorems too)
-theorem count_pos_sublist {c₁ c₂ : clause} : c₁ <+ c₂ → count_pos c₁ ≤ count_pos c₂ := 
-assume h, by simp [count_pos, sublist.countp_le (λ l, is_pos l = tt) h]
+theorem count_pos_sublist {c₁ c₂ : clause V} : 
+  c₁ <+ c₂ → c₁.count_pos ≤ c₂.count_pos :=
+assume h, by simp [count_pos, sublist.countp_le literal.is_pos h]
 
-theorem count_neg_sublist {c₁ c₂ : clause} : c₁ <+ c₂ → count_neg c₁ ≤ count_neg c₂ :=
-assume h, by simp [count_neg, sublist.countp_le (λ l, is_neg l = tt) h]
+theorem count_neg_sublist {c₁ c₂ : clause V} :
+  c₁ <+ c₂ → c₁.count_neg ≤ c₂.count_neg :=
+assume h, by simp [count_neg, sublist.countp_le literal.is_neg h]
 
-theorem count_tt_sublist (α : assignment) {c₁ c₂ : clause} : c₁ <+ c₂ → count_tt α c₁ ≤ count_tt α c₂ :=
-assume h, by simp [count_tt, sublist.countp_le (λ l, literal.eval α l = tt) h]
+theorem count_tt_sublist (α : assignment V) {c₁ c₂ : clause V} :
+  c₁ <+ c₂ → c₁.count_tt α ≤ c₂.count_tt α :=
+assume h, by simp [count_tt, sublist.countp_le (literal.is_true α) h]
 
-theorem count_ff_sublist (α : assignment) {c₁ c₂ : clause} : c₁ <+ c₂ → count_ff α c₁ ≤ count_ff α c₂ :=
-assume h, by simp [count_ff, sublist.countp_le (λ l, literal.eval α l = ff) h]
+theorem count_ff_sublist (α : assignment V) {c₁ c₂ : clause V} :
+  c₁ <+ c₂ → c₁.count_ff α ≤ c₂.count_ff α :=
+assume h, by simp [count_ff, sublist.countp_le (literal.is_false α) h]
 
-theorem exists_pos_iff_pos_count_pos {c : clause} : count_pos c > 0 ↔ ∃ l ∈ c, is_pos l :=
+theorem pos_count_pos_iff_exists_pos {c : clause V} :
+  c.count_pos > 0 ↔ ∃ l ∈ c, literal.is_pos l :=
 by simp [count_pos, countp_pos]
 
-theorem exists_neg_iff_pos_count_neg {c : clause} : count_neg c > 0 ↔ ∃ l ∈ c, is_neg l :=
+theorem pos_count_neg_iff_exists_neg {c : clause V} :
+  c.count_neg > 0 ↔ ∃ l ∈ c, literal.is_neg l :=
 by simp [count_neg, countp_pos]
 
-theorem exists_tt_iff_pos_count_tt {α : assignment} {c : clause} : count_tt α c > 0 ↔ ∃ l ∈ c, literal.eval α l = tt :=
+theorem pos_count_tt_iff_exists_tt {α : assignment V} {c : clause V} :
+  c.count_tt α > 0 ↔ ∃ l ∈ c, literal.is_true α l :=
 by simp [count_tt, countp_pos]
 
-theorem exists_ff_iff_pos_count_ff {α : assignment} {c : clause} : count_ff α c > 0 ↔ ∃ l ∈ c, literal.eval α l = ff :=
+theorem pos_count_ff_iff_exists_ff {α : assignment V} {c : clause V} :
+  c.count_ff α > 0 ↔ ∃ l ∈ c, literal.is_false α l :=
 by simp [count_ff, countp_pos]
 
 /-! # Flip counting -/
 
--- Flip counting
--- Not good from a set perspective, as order must be maintained
-def count_flips : clause → clause → nat
+-- If two clauses have the same length, literals can be compared at each
+-- position. If they are literal.flip's of each other, increment a counter
+
+-- Note: not good from a set perspective, as order must be maintained
+
+def count_flips : clause V → clause V → nat
 | []         _        := 0
 | _         []        := 0
-| (l :: ls) (m :: ms) := ite (l.flip = m) (1 + count_flips ls ms) (count_flips ls ms)
+| (l :: ls) (m :: ms) := ite (l.flip = m) 
+                         (1 + count_flips ls ms) (count_flips ls ms)
 
-@[simp] lemma count_flips_nil (c₁ c₂ : clause) : c₁ = [] ∨ c₂ = [] → count_flips c₁ c₂ = 0 :=
+@[simp] lemma count_flips_nil (c₁ c₂ : clause V) : 
+  c₁ = [] ∨ c₂ = [] → count_flips c₁ c₂ = 0 :=
 begin
   intro h, rcases h with rfl | rfl, 
   { cases c₂; { simp [count_flips] } },
   { cases c₁; { simp [count_flips] } }
 end
 
-theorem count_flips_cons (c₁ c₂ : clause) (l₁ l₂ : literal) :
-  count_flips (l₁ :: c₁) (l₂ :: c₂) = bool.to_nat (l₁.flip = l₂) + count_flips c₁ c₂ :=
-by { by_cases l₁.flip = l₂; simp [count_flips, h, bool.to_nat] }
+theorem count_flips_cons (c₁ c₂ : clause V) (l₁ l₂ : literal V) :
+  count_flips (l₁ :: c₁) (l₂ :: c₂) = ite (l₁.flip = l₂) 
+    (1 + count_flips c₁ c₂) (count_flips c₁ c₂) :=
+by { by_cases l₁.flip = l₂; simp [count_flips, h] }
 
-lemma count_flips_self (c : clause) : count_flips c c = 0 :=
+theorem count_flips_self (c : clause V) : count_flips c c = 0 :=
 begin
   induction c with l ls ih,
   { simp },
   { simp [count_flips, flip_ne, ih] }
 end
 
-lemma count_flips_comm (c₁ : clause) : ∀ (c₂ : clause), count_flips c₁ c₂ = count_flips c₂ c₁ :=
+lemma count_flips_comm (c₁ c₂ : clause V) : 
+  count_flips c₁ c₂ = count_flips c₂ c₁ :=
 begin
-  induction c₁ with l ls ih,
+  induction c₁ with l ls ih generalizing c₂,
   { simp },
-  { intro c₂, cases c₂,
-    { simp [count_flips] },
+  { cases c₂,
+    { unfold count_flips },
     { simp [count_flips, ih c₂_tl],
-      cases classical.em (l.flip = c₂_hd),
-      { simp [h, (congr_arg literal.flip h).symm], rw flip_flip l, simp },
-      { have : l.flip.flip ≠ c₂_hd.flip, from flip_injective.ne h,
-        rw flip_flip at this,
-        simp [h, (ne.symm this)] } } }
+      by_cases h : (l.flip = c₂_hd),
+      { simp [h, flip_eq_iff_eq_flip.mp h, flip_flip] },
+      { simp [h, ne.symm (flip_ne_iff_ne_flip.mp h), flip_flip] } } }
 end
 
-theorem count_flips_pos_of_neq_of_map_var_eq {c₁ : clause} :
-  ∀ {c₂ : clause}, map var c₁ = map var c₂ → c₁ ≠ c₂ → count_flips c₁ c₂ > 0 :=
+theorem count_flips_pos_of_map_var_eq_of_neq {c₁ c₂ : clause V} :
+  map var c₁ = map var c₂ → c₁ ≠ c₂ → count_flips c₁ c₂ > 0 :=
 begin
-  induction c₁ with l ls ih,
-  { intros c₂ h,
-    simp at h,
-    simp [eq_nil_of_map_eq_nil h.symm] },
-  { intros c₂ h hneq,
-    rcases exists_cons_of_map_cons h.symm with ⟨x, xs, rfl, hxl, hxs⟩,
-    by_cases heq : l = x,
-    { simp [count_flips, ih hxs.symm (ne_tail_of_eq_head_of_ne hneq heq), heq, flip_ne] },
-    { rcases eq_or_flip_eq_of_var_eq hxl.symm with rfl | hlf,
-      { contradiction },
-      { simp [count_flips, nat.zero_lt_one_add, hlf] } } }
+  induction c₁ with l ls ih generalizing c₂,
+  { intros h₁ h₂,
+    exact absurd (eq_nil_of_map_eq_nil h₁.symm).symm h₂ },
+  { intros h hne,
+    rcases exists_map_cons_of_map_cons h.symm with ⟨x, xs, rfl, hxl, hxs⟩,
+    unfold count_flips,
+    rcases var_eq_iff_eq_or_flip_eq.mp hxl with rfl | rfl,
+    { simp [ih (tail_eq_of_cons_eq h) (ne_tail_of_eq_head_of_ne hne rfl)] },
+    { simp [flip_flip, nat.zero_lt_one_add] } }
 end
 
-theorem count_flips_falsify_eq_count_tt (α : assignment) (c : clause) :
+theorem count_flips_falsify_eq_count_tt (α : assignment V) (c : clause V) :
   count_flips c (falsify α (map var c)) = count_tt α c :=
 begin
   induction c with l ls ih,
   { simp },
-  { cases l; { cases h : (α l);
-    { simp [falsify, count_flips, h, var, literal.flip, count_tt_cons, bool.to_nat, literal.eval, ih] } } }
+  { cases l;
+    { cases h : (α l);
+      { simp [map_cons, falsify_cons, count_tt_cons, count_flips_cons, 
+          literal.eval, h, var, literal.flip, ih] } } }
 end
 
 /-! ## Parity reasoning for evaluation -/
 
--- This can probably be vastly shortened with a restatement or the introduction with a few supporting lemmas
-theorem eval_tt_of_neq_counts {α : assignment} {ns : list nat} (hnil : ns ≠ []) :
-  ∀ (c : clause), map var c = ns → count_tt α (map Pos ns) ≠ count_neg c → clause.eval α c = tt :=
+theorem eval_tt_of_tt_ne_neg_of_map_var_eq 
+  {α : assignment V} {l : list V} {c : clause V} :
+  map var c = l → count_tt α (map Pos l) ≠ count_neg c → c.eval α = tt :=
 begin
-  induction ns with m ms ih,
-  { contradiction },
-  { cases ms,
-    { intros c hc hne,
-      rcases exists_of_map_singleton hc with ⟨l, rfl, hl⟩,
-      cases l; simp [is_neg, bool.to_nat] at hne; simp only [var] at hl,
-      { simp [hl, cond_tt_of_not_cond_eq_second_of_ne (literal.eval α (Pos m)) one_ne_zero hne] },
-      { have := cond_ff_of_not_cond_eq_first_of_ne (literal.eval α (Pos m)) zero_ne_one hne,
-        simp [literal.eval] at this,
-        simp [this, literal.eval, hl] } },
-    { intros c hc hcount,
-      rcases exists_cons_of_map_cons hc with ⟨l, ls, rfl, hl, hls⟩,
-      have ihred := ih (cons_ne_nil ms_hd ms_tl) ls hls,
-      cases l; rw var at hl,
-      { cases h : (α m),
-        { rw [map_cons, count_tt_cons] at hcount,
-          simp only [count_neg_cons, literal.eval, h, is_neg, bool.to_nat, cond, zero_add] at hcount,
-          exact eval_tt_cons_of_eval_tt (Pos l) (ihred hcount) },
-        { simp [eval_cons, literal.eval, h, hl] } },
-      { cases h : (α m),
-        { simp [eval_cons, literal.eval, h, hl] },
-        { rw [map_cons, count_tt_cons] at hcount,
-          simp only [count_neg_cons, literal.eval, h, is_neg, bool.to_nat, cond] at hcount,
-          exact eval_tt_cons_of_eval_tt (Neg l) (ihred (ne_of_apply_ne (has_add.add 1) hcount)) } } } }
+  induction l with v vs ih generalizing c,
+  { rw map_eq_nil, rintro rfl, contradiction },
+  { intros hc hne,
+    rcases exists_cons_of_map_cons hc with ⟨l, ls, rfl, hl, hls⟩,
+    cases l,
+    { cases h : α v,
+      { simp [map_cons, count_tt_cons, count_neg_cons, 
+          literal.is_neg, literal.eval, h] at hne,
+        exact eval_tt_cons_of_eval_tt _ (ih hls hne) },
+      { unfold var at hl,
+        simp [eval_cons, literal.eval, h, hl] } },
+    { cases h : α v,
+      { unfold var at hl,
+        simp [eval_cons, literal.eval, h, hl] },
+      { simp [map_cons, count_tt_cons, count_neg_cons, 
+          literal.is_neg, literal.eval, h] at hne,
+        exact eval_tt_cons_of_eval_tt _ (ih hls hne) } } }
 end
 
--- Basically the same proof here - shorten the above one, shorten this one
--- Take complement of the ≠ statement with length c to get the premises of the above?
-theorem eval_tt_of_neq_counts2 {α : assignment} {ns : list nat} (hnil : ns ≠ []) :
-  ∀ (c : clause), map var c = ns → count_ff α (map Pos ns) ≠ count_pos c → clause.eval α c = tt :=
+-- Basically the same proof here as the one above
+-- Take complement of count_ff, etc. to get above premises?
+theorem eval_tt_of_ff_ne_pos_of_map_var_eq 
+  {α : assignment V} {l : list V} {c : clause V} :
+  map var c = l → count_ff α (map Pos l) ≠ count_pos c → c.eval α = tt :=
 begin
-  induction ns with m ms ih,
-  { contradiction },
-  { cases ms;
-    intros c hc hne,
-    { rcases exists_of_map_singleton hc with ⟨l, rfl, hl⟩,
-      cases l; simp [is_pos, bool.to_nat] at hne; simp only [var] at hl,
-      { have := cond_tt_of_not_cond_eq_second_of_ne (literal.eval α (Pos m)) zero_ne_one hne,
-        simp [literal.eval] at this,
-        simp [hl, this, literal.eval] },
-      { have := cond_ff_of_not_cond_eq_first_of_ne (literal.eval α (Pos m)) one_ne_zero hne,
-        simp [literal.eval] at this,
-        simp [this, literal.eval, hl] } },
-    { rcases exists_cons_of_map_cons hc with ⟨l, ls, rfl, hl, hls⟩,
-      have ihred := ih (cons_ne_nil ms_hd ms_tl) ls hls,
-      cases l; rw var at hl,
-      { cases h : (α m),
-        { rw [map_cons, count_ff_cons] at hne,
-          simp only [count_pos_cons, literal.eval, h, is_pos, bool.to_nat, cond, bnot] at hne,
-          exact eval_tt_cons_of_eval_tt (Pos l) (ihred (ne_of_apply_ne (has_add.add 1) hne)) },
-        { simp [eval_cons, literal.eval, h, hl] } },
-      { cases h : (α m),
-        { simp [eval_cons, literal.eval, h, hl] },
-        { rw [map_cons, count_ff_cons] at hne,
-          simp only [count_neg_cons, literal.eval, h, is_pos, bool.to_nat, cond, bnot, zero_add] at hne,
-          exact eval_tt_cons_of_eval_tt (Neg l) (ihred hne) } } } }
+  induction l with v vs ih generalizing c,
+  { rw map_eq_nil, rintro rfl, contradiction },
+  { intros hc hne,
+    rcases exists_cons_of_map_cons hc with ⟨l, ls, rfl, hl, hls⟩,
+    cases l,
+    { cases h : α v,
+      { simp [map_cons, count_ff_cons, count_pos_cons, 
+          literal.is_pos, literal.eval, h] at hne,
+        exact eval_tt_cons_of_eval_tt _ (ih hls hne) },
+      { unfold var at hl,
+        simp [eval_cons, literal.eval, h, hl] } },
+    { cases h : α v,
+      { unfold var at hl,
+        simp [eval_cons, literal.eval, h, hl] },
+      { simp [map_cons, count_ff_cons, count_pos_cons, 
+          literal.is_pos, literal.eval, h] at hne,
+        exact eval_tt_cons_of_eval_tt _ (ih hls hne) } } }
 end
 
 -- Corollary of the above wrt parity reasoning
-theorem eval_tt_of_opposite_parity {α : assignment} {ns : list nat} {c : clause} (hnil : ns ≠ nil) : 
-  map var c = ns → nat.bodd (count_tt α (map Pos ns)) ≠ nat.bodd (count_neg c) → clause.eval α c = tt :=
-assume hc hcount, eval_tt_of_neq_counts hnil c hc (ne_of_apply_ne nat.bodd hcount)
+theorem eval_tt_of_opposite_parity 
+  {α : assignment V} {l : list V} {c : clause V} :
+  map var c = l → nat.bodd (count_tt α (map Pos l)) ≠ nat.bodd (count_neg c) 
+    → clause.eval α c = tt :=
+assume hc hcount, 
+  eval_tt_of_tt_ne_neg_of_map_var_eq hc (ne_of_apply_ne nat.bodd hcount)
 
 -- Parity reasoning based on flips rather than negs
 -- If a clause evaluates to false, then any clause that can be made by flipping a
 -- variable in that clause will evaluate to true
--- Shorten without much cases? Develop new tactic for symmetric casework?
-theorem eval_tt_of_neq_flips {α : assignment} {c₁ : clause} (hc₁ : c₁ ≠ []) :
-  ∀ (c₂ : clause), map var c₁ = map var c₂ → count_tt α c₁ ≠ count_flips c₁ c₂ → clause.eval α c₂ = tt :=
+theorem eval_tt_of_neq_flips {α : assignment V} {c₁ c₂ : clause V} :
+  map var c₁ = map var c₂ → 
+    count_tt α c₁ ≠ count_flips c₁ c₂ → c₂.eval α = tt :=
 begin
-  induction c₁ with l ls ih,
-  { contradiction },
-  { cases ls;
-    intros c₂ hc₂ hcount,
-    { rcases exists_of_map_singleton hc₂.symm with ⟨n, rfl, hn⟩,
-      cases h : (α l.var),
+  induction c₁ with l ls ih generalizing c₂,
+  { simp },
+  { intros hc₂ hne,
+    rcases exists_map_cons_of_map_cons hc₂.symm with ⟨m, ms, rfl, hm, hms⟩,
+    cases m,
+    { cases h : (α m),
       { cases l;
-        rw var at h; 
-        { cases n; rw [var, var] at hn,
-          { simp [h, bool.to_nat, literal.eval, count_flips, literal.flip, hn] at hcount,
-            contradiction },
-          { simp [literal.eval, h, hn] } } },
+        { unfold var at hm,
+          simp [count_tt_cons, count_flips_cons, 
+            literal.eval, literal.flip, ← hm, h] at hne,
+          exact eval_tt_cons_of_eval_tt _ (ih hms.symm hne) } },
+      { simp only [eval_cons, literal.eval, hm, h, tt_bor] } },
+    { cases h : (α m),
+      { simp only [eval_cons, literal.eval, hm, h, bnot, tt_bor] },
       { cases l;
-        rw var at h;
-        { cases n; rw [var, var] at hn,
-          { simp [literal.eval, h, hn] },
-          { simp [h, bool.to_nat, literal.eval, count_flips, literal.flip, hn] at hcount,
-            contradiction } } } },
-    { rcases exists_map_cons_of_map_cons hc₂.symm with ⟨m, ms, rfl, hm, hms⟩,
-      have ihred := ih (cons_ne_nil ls_hd ls_tl) ms hms.symm,
-      cases h : (literal.eval α m),
-      { by_cases he : l = m; rw count_tt_cons at hcount,
-        { simp [h, he, count_flips_cons, bool.to_nat] at hcount,
-          exact eval_tt_cons_of_eval_tt m (ihred hcount) },
-        { have := eval_flip_of_eval h,
-          simp [h, flip_eq_of_ne_of_var_eq (ne.symm he) hm] at this,
-          simp [h, flip_eq_of_ne_of_var_eq he hm.symm, 
-            count_flips_cons, bool.to_nat, this] at hcount,
-          exact eval_tt_cons_of_eval_tt m (ihred hcount) } },
-      { simp [eval_cons, h] } } }
+        { unfold var at hm,
+          simp [count_tt_cons, count_flips_cons, 
+            literal.eval, literal.flip, ← hm, h] at hne,
+          exact eval_tt_cons_of_eval_tt _ (ih hms.symm hne) } } } }
 end
 
-/-! # Clause variables -/
+/-! # vars -/
 
-/- Consider changing the implementation to a (fin)set
+-- Extract the set of variables in the clause
+-- As all properties are set-like properties, use a finset
 
-    The motivation for this is twofold
-      1. Hide the implementation of clause as a list. Accessing the variables of the clause
-         via the below function makes it so that (map var c) doesn't produce the same
-      2. Allow for the same in cnf, etc.
--/
+protected def vars : clause V → finset V
+| []        := ∅
+| (l :: ls) := {l.var} ∪ (vars ls) -- Use insert instead?
 
-def vars : clause → list nat
-| []        := []
-| (l :: ls) := if l ∈ ls ∨ l.flip ∈ ls then vars ls else l.var :: vars ls
+@[simp] theorem vars_nil : clause.vars ([] : clause V) = ∅ := rfl
 
-@[simp] theorem vars_nil : vars [] = [] := rfl
+@[simp] theorem vars_singleton (l : literal V) : 
+  clause.vars [l] = {l.var} :=
+by { unfold clause.vars, rw finset.union_empty }
 
-@[simp] theorem vars_singleton (l : literal) : vars [l] = [l.var] := 
-by simp [vars]
+theorem mem_vars_cons_of_mem_vars {c : clause V} (l : literal V) {v : V} : 
+  v ∈ c.vars → v ∈ clause.vars (l :: c) :=
+assume h, finset.mem_union.mpr (or.inr h)
 
-theorem mem_vars_cons_of_mem_vars {c : clause} (l : literal) : 
-  ∀ {n : nat}, n ∈ vars c → n ∈ vars (l :: c) :=
-assume n hn, by { by_cases (l ∈ c ∨ l.flip ∈ c); simp [vars, h, hn] }
-
--- This one can probably be cleaned up with a lemma
-theorem mem_vars_of_mem_clause {c : clause} : ∀ {l : literal}, l ∈ c → l.var ∈ vars c :=
+theorem mem_vars_of_mem_clause {c : clause V} {l : literal V} : 
+  l ∈ c → l.var ∈ c.vars :=
 begin
   induction c with d ds ih,
   { simp },
-  { intros l hl,
+  { intro hl,
     rcases eq_or_ne_mem_of_mem hl with rfl | hm,
-    { rcases classical.em (l ∈ ds ∨ l.flip ∈ ds) with ⟨hds | hfds⟩ | h,
-      { simp [ih hds, vars, hds], },
-      { exact flip_var_eq l ▸ mem_vars_cons_of_mem_vars l (ih hfds) },
-      { simp [h, vars] } },
-    { exact mem_vars_cons_of_mem_vars d (ih hm.2) } }
+    { exact finset.mem_union.mpr (or.inl (finset.mem_singleton_self l.var)) },
+    { exact finset.mem_union.mpr (or.inr (ih hm.2)) } }
 end
 
--- Seems a little lengthy in casework
-theorem exists_mem_clause_of_mem_vars {c : clause} {n : nat} : 
-  n ∈ vars c → ∃ (l : literal), l ∈ c ∧ l.var = n :=
+theorem exists_mem_clause_of_mem_vars {c : clause V} {v : V} : 
+  v ∈ c.vars → ∃ (l : literal V), l ∈ c ∧ l.var = v :=
 begin
   induction c with l ls ih,
   { simp },
-  { by_cases (l ∈ ls ∨ l.flip ∈ ls),
-    { simp [h, vars],
-      intro hn,
-      rcases ih hn with ⟨m, hm, hms⟩,
-      use m, simp [hm, hms] },
-    { simp [h, vars],
-      rintros (hn | hn),
-      { use l, simp [hn] },
-      { rcases ih hn with ⟨m, hm, hms⟩,
-        use m, simp [hm, hms] } } }
+  { intro hmem, 
+    by_cases h : (l.var = v),
+    { use [l, mem_cons_self l ls, h] },
+    { rcases finset.mem_union.mp hmem with h₁| h₂,
+      { exact absurd (finset.mem_singleton.mp h₁).symm h },
+      { rcases ih h₂ with ⟨m, hm, hv⟩,
+        use [m, mem_cons_of_mem l hm, hv] } } }
 end
 
-theorem vars_subset_of_vars_cons (c : clause) (l : literal) :
-  vars c ⊆ vars (l :: c) :=
-by { by_cases (l ∈ c ∨ l.flip ∈ c); simp [vars, h] }
+theorem vars_subset_of_vars_cons (l : literal V) (c : clause V) :
+  c.vars ⊆ clause.vars (l :: c) :=
+finset.subset_union_right _ _
 
--- Unsurprisingly, (map var c) and vars c are equivalent from a set perspective
-theorem vars_subset_of_map_var : ∀ (c : clause), vars c ⊆ map var c
-| []        := by simp
-| (l :: ls) := assume n hn, mem_map.mpr (exists_mem_clause_of_mem_vars hn)
+theorem vars_subset_of_subset {c₁ c₂ : clause V} :
+  c₁ ⊆ c₂ → c₁.vars ⊆ c₂.vars :=
+begin
+  intros h v hv,
+  rcases exists_mem_clause_of_mem_vars hv with ⟨l, hl, rfl⟩,
+  exact mem_vars_of_mem_clause (h hl)
+end
 
-theorem map_var_subset_of_vars : ∀ (c : clause), map var c ⊆ vars c
-| []        := by simp
-| (l :: ls) := assume n hn, by 
-  { rcases mem_map.mp hn with ⟨l, hl, hls⟩, exact hls ▸ mem_vars_of_mem_clause hl }
+-- (map var c) and vars c are equivalent from a set perspective
+theorem mem_vars_iff_mem_map_vars {c : clause V} {v : V} :
+  v ∈ c.vars ↔ v ∈ map var c :=
+begin
+  split,
+  { intro h,
+    exact mem_map.mpr (exists_mem_clause_of_mem_vars h) },
+  { intro h,
+    rcases mem_map.mp h with ⟨l, hmem, hv⟩,
+    exact hv ▸ mem_vars_of_mem_clause hmem }
+end
 
-theorem mem_vars_iff_mem_map_vars {c : clause} {n : nat} :
-  n ∈ map var c ↔ n ∈ vars c :=
-⟨λ h, map_var_subset_of_vars c h, λ h, vars_subset_of_map_var c h⟩
-
-theorem not_mem_vars_iff_not_mem_map_vars {c : clause} {n : nat} :
-  n ∉ map var c ↔ n ∉ vars c :=
+theorem not_mem_vars_iff_not_mem_map_vars {c : clause V} {v : V} :
+  v ∉ map var c ↔ v ∉ c.vars :=
 by simp [mem_vars_iff_mem_map_vars]
 
--- Premises can be curried, but and_imp is being troublesome
-theorem not_mem_vars_of_not_mem_clause {c : clause} {l : literal} : 
-  l ∉ c ∧ l.flip ∉ c → l.var ∉ vars c :=
+theorem mem_vars_iff_pos_or_neg_mem_clause {c : clause V} {v : V} :
+  v ∈ c.vars ↔ (Pos v) ∈ c ∨ (Neg v) ∈ c :=
+begin
+  split,
+  { intro h,
+    rcases exists_mem_clause_of_mem_vars h with ⟨l, hmem, hv⟩,
+    cases l; { rw ← hv, simp [var, hmem] } },
+  { rintros (h | h);
+    { exact mem_vars_of_mem_clause h } }
+end
+
+theorem vars_append_subset_left (c₁ c₂ : clause V) :
+  clause.vars c₁ ⊆ clause.vars (c₁ ++ c₂) :=
+begin
+  intros v hv,
+  rcases mem_vars_iff_pos_or_neg_mem_clause.mp hv with hv | hv;
+  { have := mem_vars_of_mem_clause (mem_append_left _ hv),
+    assumption },
+end
+
+theorem vars_append_subset_right (c₁ c₂ : clause V) :
+  clause.vars c₂ ⊆ clause.vars (c₁ ++ c₂) :=
+begin
+  intros v hv,
+  rcases mem_vars_iff_pos_or_neg_mem_clause.mp hv with hv | hv;
+  { have := mem_vars_of_mem_clause (mem_append_right _ hv),
+    assumption },
+end
+
+theorem mem_vars_append_left {v : V} {c₁ : clause V} (c₂ : clause V) :
+  v ∈ clause.vars c₁ → v ∈ clause.vars (c₁ ++ c₂) :=
+assume h, vars_append_subset_left c₁ c₂ h
+
+theorem mem_vars_append_right {v : V} (c₁ : clause V) {c₂ : clause V} :
+  v ∈ clause.vars c₂ → v ∈ clause.vars (c₁ ++ c₂) :=
+assume h, vars_append_subset_right c₁ c₂ h
+
+theorem mem_left_or_right_of_mem_vars_append {v : V} {c₁ c₂ : clause V} :
+  v ∈ clause.vars (c₁ ++ c₂) → (v ∈ clause.vars c₁) ∨ (v ∈ clause.vars c₂) :=
+begin
+  intro h,
+  rcases exists_mem_clause_of_mem_vars h with ⟨l, hl, rfl⟩,
+  rcases mem_append.mp hl with hl | hl;
+  { simp [mem_vars_of_mem_clause hl] }
+end
+
+theorem not_mem_vars_append_left {v : V} {c₁ c₂ : clause V} :
+  v ∉ clause.vars (c₁ ++ c₂) → v ∉ clause.vars c₁ :=
 begin
   contrapose,
   simp,
-  intros hv hc,
-  rcases exists_mem_clause_of_mem_vars hv with ⟨m, hm, hms⟩,
-  exact (flip_eq_of_ne_of_var_eq 
-    (ne.symm (ne_of_mem_of_not_mem hm hc)) hms.symm).symm ▸ hm
+  exact mem_vars_append_left c₂
 end
 
-theorem vars_nodup (c : clause) : c.vars.nodup :=
+theorem not_mem_vars_append_right {v : V} {c₁ c₂ : clause V} :
+  v ∉ clause.vars (c₁ ++ c₂) → v ∉ clause.vars c₂ :=
 begin
-  induction c with l ls ih,
-  { simp },
-  { simp [vars],
-    rcases (classical.em (l ∈ ls ∨ l.flip ∈ ls)) with ⟨hls | hls⟩ | h,
-    repeat { simp [hls, ih] },
-    { simp [h, ih], 
-      simp [not_or_distrib] at h,
-      rcases h with ⟨h1, h2⟩,
-      exact not_mem_vars_of_not_mem_clause (and.intro h1 h2) } }
+  contrapose,
+  simp,
+  exact mem_vars_append_right c₁
 end
 
-def reduced : clause → clause
-| []        := []
-| (l :: ls) := if l ∈ ls then reduced ls else l :: reduced ls
-
--- TODO can probably be implemented in terms of foldl, foldr
--- TODO Borrow the min_max list derivations for streamlining? Options aren't fun though
-def max_var : clause → nat
-| []        := 0
-| (l :: ls) := max l.var (max_var ls)
-
--- Carry over a lot of these things for min too
-@[simp] lemma max_var_nil : max_var [] = 0 := rfl
-
-@[simp] lemma max_var_singleton (l : literal) : max_var [l] = l.var :=
-by simp [max_var]
-
-lemma max_var_cons (c : clause) (l : literal) : max_var (l :: c) = max l.var (max_var c) := rfl
-
-lemma max_var_concat (c : clause) (l : literal) : max_var (c ++ [l]) = max (l.var) (max_var c) :=
+theorem not_mem_vars_append_of_not_mem_of_not_mem {v : V} {c₁ c₂ : clause V} :
+  v ∉ clause.vars c₁ → v ∉ clause.vars c₂ → v ∉ clause.vars (c₁ ++ c₂) :=
 begin
-  induction c with d ds ih,
-  { simp },
-  { simp [max_var, ih],
-    rw ← max_assoc,
-    rw ← max_assoc,
-    rw max_comm d.var l.var }
+  intros h₁ h₂ hcon,
+  rcases mem_left_or_right_of_mem_vars_append hcon with hv | hv;
+  { contradiction }
 end
-
-lemma max_var_append (c₁ c₂ : clause) : max_var (c₁ ++ c₂) = max (max_var c₁) (max_var c₂) :=
-begin
-  induction c₁ with d ds ih,
-  { simp },
-  { simp [max_var, ih],
-    rw ← max_assoc }
-end
-
-lemma max_var_le_max_var_cons (c : clause) (l : literal) : max_var c ≤ max_var (l :: c) :=
-by simp [max_var_cons]
-
-lemma max_var_lit_le_max_var_cons (c : clause) (l : literal) : max_var [l] ≤ max_var (l :: c) :=
-by simp [max_var]
-
-lemma max_var_cons_eq_max_var_of_le (c : clause) (l : literal) : l.var ≤ max_var c → max_var (l :: c) = max_var c :=
-assume h, by simp [max_var, h]
-
-lemma max_var_cons_eq_max_var_of_gt (c : clause) (l : literal) : l.var > max_var c → max_var (l :: c) = l.var :=
-begin
-  simp [max_var_cons],
-  intro h,
-  exact le_of_lt h
-end
-
--- hehe not an induction argument
-lemma sublist_lemma {α : Type} [decidable_eq α] {a : α} {l₁ l₂ : list α} : 
-  l₁ <+ (a :: l₂) → l₁ <+ l₂ ∨ (∃ b L, l₁ = b :: L ∧ a = b ∧ L <+ l₂) :=
-begin
-  induction l₁ with x xs ih,
-  { simp },
-  { intro h,
-    by_cases heq : a = x,
-    { right,
-      rw heq at h,
-      use [x, xs],
-      simp [heq, sublist_of_cons_sublist_cons h] },
-    { left,
-      cases h,
-      { assumption },
-      { contradiction } } }
-end
-
--- This seems a sort of thing a maximum or minimum has a theorem for already
-lemma max_var_sublist (c₁ : clause) : ∀ {c₂ : clause}, c₂ <+ c₁ → max_var c₂ ≤ max_var c₁ :=
-begin
-  induction c₁ with l ls ih,
-  { simp },
-  { intros c₂ hc₂,
-    rcases sublist_lemma hc₂ with hls | ⟨c, cs, rfl, rfl, hcs⟩,
-    { exact le_trans (ih hls) (max_var_le_max_var_cons ls l) },
-    { unfold max_var,
-      have ihred := ih hcs,
-      simp [ihred],
-      by_cases max_var cs ≤ l.var,
-      { left, assumption },
-      { right,
-        simp at h,
-        exact le_trans (le_of_lt h) ihred } } }
-end
-
--- Overly situational, I know
-lemma max_var_sublist_append {c₁ c₂ : clause} : ∀ {c₃ : clause}, 
-  c₃ <+ c₁ → max_var c₂ > max_var c₁ → max_var (c₃ ++ c₂) = max_var c₂ :=
-begin
-  induction c₁ with d ds ih,
-  { simp },
-  { intros c₃ hc3 hmax,
-    have hcds : c₂.max_var > max_var ds, from gt_of_gt_of_ge hmax (max_var_le_max_var_cons ds d),
-    rcases sublist_lemma hc3 with hds | ⟨a, as, rfl, rfl, has⟩,
-    { exact ih hds hcds },
-    { have ihred := ih has hcds,
-      have : d.var ≤ max_var c₂,
-      { by_contradiction,
-        simp at h,
-        have : c₂.max_var > max_var [d], from gt_of_gt_of_ge hmax (max_var_lit_le_max_var_cons ds d),
-        simp [max_var] at this,
-        have : d.var ≤ c₂.max_var, from le_of_lt this,
-        have : ¬(d.var > c₂.max_var), simp [this],
-        exact absurd h this },
-      rw ← ihred,
-      rw ← ihred at this,
-      exact max_var_cons_eq_max_var_of_le (as ++ c₂) d this } }
-end
-
-lemma forall_max_var {c : clause} {n : nat} : c ≠ [] → n = max_var c → ∀ l ∈ c, literal.var l ≤ n :=
-begin
-  induction c with d ds ih,
-  { contradiction },
-  { intro hnil,
-    intros hn l hl,
-    have : [l] <+ d :: ds, from singleton_sublist.mpr hl,
-    rw hn,
-    exact max_var_sublist (d :: ds) this }
-end
-
-theorem not_mem_of_gt_max_var {c : clause} {l : literal} : l.var > max_var c → l ∉ c :=
-begin
-  induction c with d ds ih,
-  { simp },
-  { intro h,
-    simp [max_var] at h,
-    rcases h with ⟨hd, hds⟩,
-    have : d ≠ l, from ne_of_apply_ne (λ (d : literal), d.var) (ne_of_lt hd),
-    simp [ne.symm this, ih hds] }
-end
-
-theorem not_mem_map_var_of_gt_max_var {c : clause} {l : literal} : l.var > max_var c → l.var ∉ (map var c) :=
-begin
-  induction c with d ds ih,
-  { simp },
-  { intro h,
-    simp [max_var] at h,
-    rcases h with ⟨hd, hds⟩,
-    simp [hd, ih hds, ne_of_gt hd] }
-end
-
--- Weird proof
-theorem not_mem_map_var_of_gt_max_var2 {c : clause} {n : nat} : n > max_var c → n ∉ (map var c) :=
-begin
-  intro h,
-  have pos : (Pos n).var = n, simp [var],
-  rw ← pos at h,
-  have := not_mem_map_var_of_gt_max_var h,
-  rw pos at this,
-  exact this
-end
-
-theorem not_mem_vars_of_gt_max_var {c : clause} {l : literal} : l.var > max_var c → l.var ∉ c.vars :=
-assume h, not_mem_vars_iff_not_mem_map_vars.mp (not_mem_map_var_of_gt_max_var h)
 
 end clause
 
@@ -869,7 +772,7 @@ open list
 open literal
 open clause
 
-theorem eval_eq_of_equiv_on_clause {α₁ α₂ : assignment} {c : clause} :
+theorem eval_eq_of_eqod_on_map_var {α₁ α₂ : assignment V} {c : clause V} :
   (α₁ ≡[map var c]≡ α₂) → clause.eval α₁ c = clause.eval α₂ c :=
 begin
   intro heq,
@@ -884,8 +787,9 @@ begin
     exact hlt ▸ eval_eq_of_mem_of_eqod heq (mem_map_of_mem var hl) }
 end
 
-theorem eval_eq_of_equiv_on_clause2 {α₁ α₂ : assignment} {c : clause} :
-  (α₁ ≡[vars c]≡ α₂) → clause.eval α₁ c = clause.eval α₂ c :=
-assume h, eval_eq_of_equiv_on_clause (eqod_subset_of_eqod (map_var_subset_of_vars c) h)
+-- TODO: Think about typing here
+--theorem eval_eq_of_eqod_on_vars {α₁ α₂ : assignment V} {c : clause V} :
+--  (α₁ ≡[c.vars.to_list]≡ α₂) → clause.eval α₁ c = clause.eval α₂ c :=
+--assume h, eval_eq_of_eqod_on_map_var (eqod_subset_of_eqod (map_var_subset_of_vars c) h)
 
 end assignment
