src/cnf/cnf.lean
@@ -1,5 +1,6 @@
 /-
-This file contains the definitions of the conjunctive normal form. 
+This file contains the definitions of the conjunctive normal form.
+Variables are general. 
 
 Authors: Cayden Codel, Jeremy Avigad, Marijn Heule
 Carnegie Mellon University
@@ -15,56 +16,73 @@ import data.list.perm
 import init.data.nat
 import data.nat.basic
 
+universe u
+
+-- Represents the parametric type of the variable stored in the literal
+variables {V : Type u} [decidable_eq V] [inhabited V]
+
 /- Conjunctive normal form is a list of clauses joined by logical ANDs -/
-def cnf := list clause
+def cnf (V : Type u) := list (clause V)
 
 namespace cnf
 
 open literal
 open clause
 open list
+open function 
 
 /-! # Instance properties -/
 
-instance : inhabited cnf := ⟨[default clause]⟩
-instance : has_mem clause cnf := ⟨list.mem⟩
-instance : has_emptyc cnf := ⟨list.nil⟩
-instance : has_union cnf := ⟨list.union⟩
-instance : has_inter cnf := ⟨list.inter⟩
-instance : has_singleton clause cnf := ⟨λ c, [c]⟩ 
-instance : has_insert clause cnf := ⟨list.insert⟩
-instance : has_append cnf := ⟨list.append⟩
-instance : has_subset cnf := ⟨list.subset⟩
+instance : inhabited (cnf V) := ⟨[default (clause V)]⟩
+instance : has_mem (clause V) (cnf V) := ⟨list.mem⟩
+instance : has_emptyc (cnf V) := ⟨list.nil⟩
+instance : has_union (cnf V) := ⟨list.union⟩
+instance : has_inter (cnf V) := ⟨list.inter⟩
+instance : has_singleton (clause V) (cnf V) := ⟨λ c, [c]⟩ 
+instance : has_insert (clause V) (cnf V) := ⟨list.insert⟩
+instance : has_append (cnf V) := ⟨list.append⟩
+instance : has_subset (cnf V) := ⟨list.subset⟩
+
+instance (c : clause V) (f : cnf V) : decidable (c ∈ f) :=
+begin
+  induction f with cl cls ih,
+  { exact decidable.false },
+  { cases ih,
+    { by_cases h : c = cl,
+      { rw h, exact decidable.is_true (mem_cons_self cl cls) },
+      { exact decidable.is_false (not_mem_cons_of_ne_of_not_mem h ih) } },
+    exact decidable.is_true (mem_cons_of_mem cl ih) }
+end
 
 /-! ### Evaluation under assignment -/
 
 /- The clauses of the CNF are joined by conjunctions, so all must evaluate to true -/
-protected def eval (α : assignment) (f : cnf) : bool :=
+protected def eval (α : assignment V) (f : cnf V) : bool :=
   f.foldr (λ c b, b && (clause.eval α c)) tt
 
-@[simp] theorem eval_nil {α : assignment} : cnf.eval α [] = tt := rfl
+@[simp] theorem eval_nil {α : assignment V} : cnf.eval α [] = tt := rfl
 
-@[simp] theorem eval_singleton {α : assignment} {c : clause} : 
+@[simp] theorem eval_singleton {α : assignment V} {c : clause V} : 
   cnf.eval α [c] = clause.eval α c :=
-by simp [cnf.eval]
+by simp only [cnf.eval, foldr, tt_band]
 
-theorem eval_cons {α : assignment} {c : clause} {f : cnf} : 
+theorem eval_cons {α : assignment V} {c : clause V} {f : cnf V} : 
   cnf.eval α (c :: f) = (clause.eval α c && cnf.eval α f) :=
-by simp [cnf.eval, bool.band_comm]
+by simp only [cnf.eval, foldr, bool.band_comm]
 
-theorem ne_nil_of_eval_ff {α : assignment} {f : cnf} :
+theorem ne_nil_of_eval_ff {α : assignment V} {f : cnf V} :
   cnf.eval α f = ff → f ≠ [] :=
 by { contrapose, simp, intro h, simp [h] }
 
-theorem eval_ff_cons_of_eval_ff {α : assignment} {f : cnf} (c : clause) :
+theorem eval_ff_cons_of_eval_ff {α : assignment V} {f : cnf V} (c : clause V) :
   cnf.eval α f = ff → cnf.eval α (c :: f) = ff :=
 by { simp [cnf.eval], intro h, simp [h] }
 
-theorem eval_append (α : assignment) (f₁ f₂ : cnf) : 
+theorem eval_append (α : assignment V) (f₁ f₂ : cnf V) : 
   cnf.eval α (f₁ ++ f₂) = cnf.eval α f₁ && cnf.eval α f₂ :=
 by { induction f₁ with c cs ih, simp, simp [eval_cons, ih] }
 
-lemma forall_clause_eval_tt_of_eval_tt {α : assignment} {f : cnf} : 
+lemma forall_clause_eval_tt_of_eval_tt {α : assignment V} {f : cnf V} : 
   cnf.eval α f = tt → ∀ c ∈ f, clause.eval α c = tt :=
 begin
   induction f with c cs ih,
@@ -74,7 +92,7 @@ begin
     exact and.intro hc (ih hcs) }
 end
 
-lemma eval_tt_of_forall_clause_eval_tt {α : assignment} {f : cnf} :
+lemma eval_tt_of_forall_clause_eval_tt {α : assignment V} {f : cnf V} :
   (∀ c ∈ f, clause.eval α c = tt) → cnf.eval α f = tt :=
 begin
   induction f with c cs ih,
@@ -84,11 +102,11 @@ begin
     simp [hc, ih he] }
 end
 
-theorem eval_tt_iff_forall_clause_eval_tt {α : assignment} {f : cnf} :
+theorem eval_tt_iff_forall_clause_eval_tt {α : assignment V} {f : cnf V} :
   cnf.eval α f = tt ↔ ∀ c ∈ f, clause.eval α c = tt :=
 ⟨forall_clause_eval_tt_of_eval_tt, eval_tt_of_forall_clause_eval_tt⟩
 
-lemma exists_clause_eval_ff_of_eval_ff {α : assignment} {f : cnf} : 
+lemma exists_clause_eval_ff_of_eval_ff {α : assignment V} {f : cnf V} : 
   cnf.eval α f = ff → ∃ c ∈ f, clause.eval α c = ff :=
 begin
   induction f with c cs ih,
@@ -100,7 +118,7 @@ begin
       use c, simp [hc1, hc2] } },
 end
 
-lemma eval_ff_of_exists_clause_eval_ff {α : assignment} {f : cnf} :
+lemma eval_ff_of_exists_clause_eval_ff {α : assignment V} {f : cnf V} :
   (∃ c ∈ f, clause.eval α c = ff) → cnf.eval α f = ff :=
 begin
   induction f with c cs ih,
@@ -111,18 +129,18 @@ begin
     { exact eval_ff_cons_of_eval_ff c (ih ⟨cl, h, heval⟩) } }
 end
 
-theorem eval_ff_iff_exists_clause_eval_ff {α : assignment} {f : cnf} :
+theorem eval_ff_iff_exists_clause_eval_ff {α : assignment V} {f : cnf V} :
   cnf.eval α f = ff ↔ ∃ c ∈ f, clause.eval α c = ff :=
 ⟨exists_clause_eval_ff_of_eval_ff, eval_ff_of_exists_clause_eval_ff⟩
 
 /-! ### Counting -/
 
 /- Counts the number of clauses which evaluate to true under some assignment -/
-def count_tt (α : assignment) (f : cnf) : nat :=
+def count_tt (α : assignment V) (f : cnf V) : nat :=
   length $ f.filter (λ c, c.eval α = tt)
 
 /- Counts the number of clauses which evaluate to false under some assignment -/
-def count_ff (α : assignment) (f : cnf) : nat :=
+def count_ff (α : assignment V) (f : cnf V) : nat :=
   length $ f.filter (λ c, c.eval α = ff)
 
 /-! ### Tseitin groundwork -/
@@ -135,49 +153,61 @@ def vars : cnf → list nat
 | (c :: cs) := list.foldr (λ v s, if v ∈ s then s else v :: s) (vars cs) (clause.vars c)
 -/
 
-def vars : cnf → list nat
+protected def vars : cnf V → list V
 | []        := []
 | (c :: cs) := (vars cs) ∪ (clause.vars c) -- I prefer the union the other way, but alas...
 
-@[simp] theorem vars_nil : vars [] = [] := rfl
+@[simp] theorem vars_nil : cnf.vars ([] : cnf V) = [] := rfl
 
-@[simp] theorem vars_singleton (c : clause) : vars [c] = clause.vars c :=
-by simp [vars, var, nil_union]
+@[simp] theorem vars_singleton (c : clause V) : cnf.vars [c] = clause.vars c :=
+by simp [cnf.vars, var, nil_union]
 
-theorem clause_vars_subset_of_mem {f : cnf} {c : clause} :
-  c ∈ f → (clause.vars c) ⊆ vars f :=
+theorem vars_append_subset_union (f₁ f₂ : cnf V) :
+  cnf.vars (f₁ ++ f₂) ⊆ cnf.vars f₁ ∪ cnf.vars f₂ :=
+begin
+  sorry
+end
+
+theorem vars_union_subset_append (f₁ f₂ : cnf V) :
+  cnf.vars f₁ ∪ cnf.vars f₂ ⊆ cnf.vars (f₁ ++ f₂) :=
+begin
+  sorry
+end
+
+theorem clause_vars_subset_of_mem {f : cnf V} {c : clause V} :
+  c ∈ f → (clause.vars c) ⊆ cnf.vars f :=
 begin
   intro h,
   induction f with d ds ih,
   { exact absurd h (not_mem_nil c) },
   { rcases eq_or_mem_of_mem_cons h with rfl | h2,
-    { simp [vars],
+    { simp [cnf.vars],
       intros a ha,
-      exact mem_union_right (vars ds) ha },
+      exact mem_union_right (cnf.vars ds) ha },
     { have ihred := ih h2,
-      unfold vars,
+      unfold cnf.vars,
       intros a ha,
       exact mem_union_left (ihred ha) (d.vars) } }
 end
 
-theorem mem_vars_of_mem_clause_of_mem {f : cnf} {c : clause} {n : nat} :
-  c ∈ f → n ∈ (clause.vars c) → n ∈ vars f :=
+theorem mem_vars_of_mem_clause_of_mem {f : cnf V} {c : clause V} {v : V} :
+  c ∈ f → v ∈ (clause.vars c) → v ∈ cnf.vars f :=
 begin
   induction f with d ds ih,
   { simp },
   { intros hc hn,
     rcases eq_or_mem_of_mem_cons hc with rfl | hds,
-    { simp [vars, hn] },
-    { simp [vars, ih hds hn] } }
+    { simp [cnf.vars, hn] },
+    { simp [cnf.vars, ih hds hn] } }
 end
 
-protected theorem exists_mem_clause_of_mem_vars {f : cnf} {n : nat} :
-  n ∈ vars f → ∃ (c : clause), c ∈ f ∧ n ∈ (clause.vars c) :=
+protected theorem exists_mem_clause_of_mem_vars {f : cnf V} {v : V} :
+  v ∈ cnf.vars f → ∃ (c : clause V), c ∈ f ∧ v ∈ (clause.vars c) :=
 begin
   induction f with c cs ih,
   { simp },
   { intro hn,
-    simp [vars] at hn,
+    simp [cnf.vars] at hn,
     rcases hn with hcs | hc,
     { rcases ih hcs with ⟨cl, hcl, hcls⟩,
       use cl,
@@ -186,20 +216,78 @@ begin
       simp [mem_cons_self c cs, hc] } }
 end
 
-theorem subset_vars_of_subset_cnf {f₁ f₂ : cnf} :
-  f₁ ⊆ f₂ → (vars f₁) ⊆ (vars f₂) :=
+theorem subset_vars_of_subset_cnf {f₁ f₂ : cnf V} :
+  f₁ ⊆ f₂ → (cnf.vars f₁) ⊆ (cnf.vars f₂) :=
 begin
   intros h n hn,
   rcases cnf.exists_mem_clause_of_mem_vars hn with ⟨c, hf, hnc⟩,
   exact mem_vars_of_mem_clause_of_mem (h hf) hnc
 end
 
-theorem exists_not_mem_vars : ∀ (f : cnf), ∃ (n : nat), n ∉ (vars f)
-| []        := by simp
-| f := begin
-  use (max_nat (vars f)) + 1,
-  exact not_mem_of_gt_max_nat (lt_add_one (max_nat (vars f))),
+theorem exists_not_mem_vars_of_bijection {g : V → nat} (hg : bijective g) (f : cnf V) :
+  ∃ (v : V), v ∉ cnf.vars f :=
+begin
+  cases f,
+  { use [(arbitrary V), not_mem_nil _] },
+  { have : foldr max 0 (map g (cnf.vars (f_hd :: f_tl))) + 1 > 
+      foldr max 0 (map g (cnf.vars (f_hd :: f_tl))),
+      from lt_add_one _,
+    rcases exists_not_mem_of_gt_max hg this with ⟨v, heq, hv⟩,
+    use [v, hv] }
 end
+
+-- Corollary of the above
+theorem exists_not_mem_forall_clause_of_bijection 
+  {g : V → nat} (hg : bijective g) (f : cnf V) :
+  ∃ (v : V), ∀ (c : clause V), c ∈ f → v ∉ clause.vars c :=
+begin
+  rcases exists_not_mem_vars_of_bijection hg f with ⟨v, hv⟩,
+  use v,
+  intros c hc hvnot,
+  have := clause_vars_subset_of_mem hc,
+  exact hv (this hvnot)
+end
+
+/-! # Equisatisfiability -/
+
+def equisatisfiable (f₁ f₂ : cnf V) :=
+  (∃ (α₁ : assignment V), cnf.eval α₁ f₁ = tt) ↔ ∃ (α₂ : assignment V), cnf.eval α₂ f₂ = tt
+
+notation f₁ ` ≈ ` f₂ := equisatisfiable f₁ f₂
+
+@[simp] theorem equisatisfiable_nil : equisatisfiable ([] : cnf V) [] :=
+by simp [equisatisfiable]
+
+@[refl] theorem equisatisfiable.refl (f : cnf V) : f ≈ f :=
+begin
+  split;
+  { rintros ⟨α, ha⟩,
+    use [α, ha] }
+end
+
+@[symm] theorem equisatisfiable.symm (f₁ f₂ : cnf V) :
+  f₁ ≈ f₂ → f₂ ≈ f₁ :=
+begin
+  unfold equisatisfiable,
+  rintros ⟨hmp, hmpr⟩,
+  exact ⟨hmpr, hmp⟩
+end
+
+@[trans] theorem equisatisfiable.trans {f₁ f₂ f₃ : cnf V} :
+  f₁ ≈ f₂ → f₂ ≈ f₃ → f₁ ≈ f₃ :=
+begin
+  rintros ⟨hmp1, hmpr1⟩ ⟨hmp2, hmpr2⟩,
+  split,
+  { intro h, exact hmp2 (hmp1 h) },
+  { intro h, exact hmpr1 (hmpr2 h) }
+end
+
+-- Can make this be an equivalence relation now
+
+/-! # Equivalence -/
+
+def equivalent (f₁ f₂ : cnf V) :=
+  ∀ (α : assignment V), cnf.eval α f₁ = cnf.eval α f₂
 
 end cnf
 
@@ -212,7 +300,7 @@ open clause
 open cnf
 open list
 
-theorem eval_eq_of_equiv_on_domain_vars {α₁ α₂ : assignment} {f : cnf} :
+theorem eval_eq_of_equiv_on_domain_vars {α₁ α₂ : assignment V} {f : cnf V} :
   (α₁ ≡[f.vars]≡ α₂) → cnf.eval α₁ f = cnf.eval α₂ f :=
 begin
   intro h,
