src/cnf/literal.lean
@@ -1,161 +1,234 @@
 /-
-
-  This file contains the definition of a Boolean literal.
-  
-  Authors: Cayden Codel, Jeremy Avigad, Marijn Heule
-  Carnegie Mellon University
-
+This file contains the definition of a Boolean literal.
+The type of the underlying Boolean variable is polymorphic, such
+that Boolean variables may be represented by nats, strings, etc.
+ 
+Authors: Cayden Codel, Jeremy Avigad, Marijn Heule
+Carnegie Mellon University
 -/
 
-import init.data.nat
-import init.logic
 import logic.function.basic
-import data.list.basic
+import tactic
 
-/- 
-  All propositional formulas are comprised of Boolean variables.
-  Here, we represent variables as natural numbers, which may then be evaluated
-  with an appropriate assignment of boolean values to those variables.
+universe u
 
-  Literals are positive and negative instances of those variables.
+-- Represents the parametric type of the variable stored in the literal
+variables {V : Type u} [decidable_eq V] [inhabited V]
+
+/-
+All propositional formulas are comprised of Boolean literals.
+Literals are positive or negative forms of the underlying variable type.
 -/
 @[derive decidable_eq]
-inductive literal : Type
-| Pos : nat → literal
-| Neg : nat → literal
+inductive literal (V)
+| Pos (v : V) : literal
+| Neg (v : V) : literal
 
-/- Assignments give boolean values to the variables -/
-def assignment := nat → bool
+/-
+Propositional formulas may be evaluated under truth assignments.
+Assignments give boolean values to the variables in the formula.
+-/
+def assignment (V : Type u) := V → bool
 
 namespace literal
 
 open function
 
-/- Instance properties -/
-instance : inhabited literal := ⟨Pos 0⟩
+/-! # Properties -/
 
-/- Extracts the natural number boolean variable of the literal -/
-def var : literal → nat
-| (Pos n) := n
-| (Neg n) := n
+instance : inhabited (literal V) := ⟨Pos (arbitrary V)⟩
 
-/- Negated literals receive the opposite boolean value as the variable -/
-protected def eval (α : assignment) : literal → bool
-| (Pos n) := α n
-| (Neg n) := bnot (α n)
+/-! # Var -/
+
+/- Extracts the underlying variable of the literal -/
+def var : literal V → V
+| (Pos v) := v
+| (Neg v) := v
+
+theorem var_surjective : surjective (var : literal V → V) :=
+assume v, exists.intro (Pos v) (by simp only [var])
+
+theorem ne_of_ne_var {l₁ l₂ : literal V} :
+  l₁.var ≠ l₂.var → l₁ ≠ l₂ :=
+assume h₁ h₂, h₁ (congr_arg var h₂)
+
+-- Cases on l gives this immediately, so a kind of shorthand
+theorem pos_or_neg_of_var_eq_nat {l : literal V} {v : V} :
+  l.var = v → l = (Pos v) ∨ l = (Neg v) :=
+begin
+  cases l,
+  { simp only [var], exact or.intro_left false },
+  { simp only [var], exact or.intro_right false }
+end
+
+/-! # Evaluation -/
+
+/-
+When provided an assignment, literals may be evaluated against
+that assignment. Negated literals flip the truth value of the
+underlying variable when evaluated on the assignment.
+-/
+protected def eval (α : assignment V) : literal V → bool
+| (Pos v) := α v
+| (Neg v) := bnot (α v)
 
 /-! # Flip -/
 
 /- Flips the parity of the literal from positive to negative and vice versa -/
-def flip : literal → literal
-| (Pos n) := Neg n
-| (Neg n) := Pos n
+-- Protected because "flip" exists already as a way to interchange
+-- the order of curried arguments
+protected def flip : literal V → literal V
+| (Pos v) := Neg v
+| (Neg v) := Pos v
 
-@[simp] theorem flip_ne (l : literal) : l.flip ≠ l :=
-by cases l; simp [flip]
+@[simp] theorem flip_ne (l : literal V) : l.flip ≠ l :=
+by cases l; unfold literal.flip; exact dec_trivial
 
-theorem flip_flip (l : literal) : l.flip.flip = l :=
-by cases l; simp only [flip]
+theorem flip_flip (l : literal V) : l.flip.flip = l :=
+by cases l; simp only [literal.flip]
 
-theorem flip_var_eq (l : literal) : l.flip.var = l.var :=
-by cases l; simp only [flip, var]
+theorem flip_var_eq (l : literal V) : l.flip.var = l.var :=
+by cases l; simp only [literal.flip, var]
 
-@[simp] theorem flip_injective : injective (literal.flip) :=
-assume l₁ l₂ h, (flip_flip l₂) ▸ ((flip_flip l₁) ▸ (congr_arg flip h))
+@[simp] theorem flip_injective : 
+  injective (literal.flip : literal V → literal V) :=
+assume l₁ l₂ h, (flip_flip l₂) ▸ ((flip_flip l₁) ▸ (congr_arg literal.flip h))
 
-theorem flip_inj {l₁ l₂ : literal} : l₁.flip = l₂.flip ↔ l₁ = l₂ :=
+theorem flip_inj {l₁ l₂ : literal V} : l₁.flip = l₂.flip ↔ l₁ = l₂ :=
 flip_injective.eq_iff
 
-@[simp] theorem flip_surjective : surjective flip :=
+@[simp] theorem flip_surjective : 
+  surjective (literal.flip : literal V → literal V) :=
 assume l, exists.intro l.flip (flip_flip l)
 
-@[simp] theorem flip_bijective : bijective flip :=
+@[simp] theorem flip_bijective : 
+  bijective (literal.flip : literal V → literal V) :=
 ⟨flip_injective, flip_surjective⟩
 
-lemma eq_or_flip_eq_of_var_eq {l₁ l₂ : literal} : 
-  l₁.var = l₂.var → l₁ = l₂ ∨ l₁.flip = l₂ :=
-by cases l₁; { cases l₂; simp [flip, var] }
+-- Various lemmas on how var and flip interact
 
-lemma var_eq_of_eq_or_flip_eq {l₁ l₂ : literal} : 
-  l₁ = l₂ ∨ l₁.flip = l₂ → l₁.var = l₂.var :=
-assume h, or.elim h
-  (assume : l₁ = l₂, congr_arg var this)
-  (assume : l₁.flip = l₂, congr_arg var this ▸ (flip_var_eq l₁).symm)
-
-theorem eq_or_flip_eq_iff_var_eq {l₁ l₂ : literal} : 
+theorem var_eq_iff_eq_or_flip_eq {l₁ l₂ : literal V} : 
   l₁.var = l₂.var ↔ l₁ = l₂ ∨ l₁.flip = l₂ :=
-⟨eq_or_flip_eq_of_var_eq, var_eq_of_eq_or_flip_eq⟩
+begin
+  split,
+  { cases l₁; { cases l₂; simp [literal.flip, var] }},
+  { intro h, cases h,
+    { exact congr_arg var h },
+    { exact congr_arg var h ▸ (flip_var_eq l₁).symm } }
+end
 
-theorem flip_eq_iff_eq_flip {l₁ l₂ : literal} : l₁.flip = l₂ ↔ l₁ = l₂.flip :=
-⟨λ h, congr_arg flip h ▸ (flip_flip l₁).symm, λ h, (congr_arg flip h).symm ▸ flip_flip l₂⟩
+theorem flip_eq_iff_eq_flip {l₁ l₂ : literal V} : 
+  l₁.flip = l₂ ↔ l₁ = l₂.flip :=
+⟨λ h, congr_arg literal.flip h ▸ (flip_flip l₁).symm, 
+ λ h, (congr_arg literal.flip h).symm ▸ flip_flip l₂⟩
 
-theorem flip_eq_of_ne_of_var_eq {l₁ l₂ : literal} :
+theorem flip_ne_iff_ne_flip {l₁ l₂ : literal V} :
+  l₁.flip ≠ l₂ ↔ l₁ ≠ l₂.flip :=
+begin
+  split;
+  { contrapose,
+    simp [flip_eq_iff_eq_flip] },
+end
+
+theorem flip_eq_of_ne_of_var_eq {l₁ l₂ : literal V} :
   l₁ ≠ l₂ → l₁.var = l₂.var → l₁.flip = l₂ :=
 begin
   intros h₁ h₂,
-  cases eq_or_flip_eq_of_var_eq h₂,
+  cases var_eq_iff_eq_or_flip_eq.mp h₂,
   { contradiction },
   { exact h }
 end
 
-theorem eq_of_flip_ne_of_var_eq {l₁ l₂ : literal} :
+theorem eq_of_flip_ne_of_var_eq {l₁ l₂ : literal V} :
   l₁.flip ≠ l₂ → l₁.var = l₂.var → l₁ = l₂ :=
 begin
   intros h₁ h₂,
-  cases eq_or_flip_eq_of_var_eq h₂,
+  cases var_eq_iff_eq_or_flip_eq.mp h₂,
   { exact h },
   { contradiction }
 end
 
 /-! # Flip evaluation -/
 
-theorem eval_flip (α : assignment) (l : literal) : 
-  literal.eval α l = bnot (literal.eval α l.flip) :=
-by cases l; simp only [flip, literal.eval, bnot_bnot]
+-- When a literal is flipped, its truth assignment is negated
+theorem eval_flip (α : assignment V) (l : literal V) : 
+  l.flip.eval α = bnot (l.eval α) :=
+by cases l; simp only [literal.flip, literal.eval, bnot_bnot]
 
-theorem eval_flip2 (α : assignment) (l : literal) : 
-  literal.eval α l.flip = bnot (literal.eval α l) :=
-by cases l; simp only [flip, literal.eval, bnot_bnot]
+-- A slight modification where the negation is the flipped literal
+theorem eval_flip2 (α : assignment V) (l : literal V) :
+  l.eval α = bnot (l.flip.eval α) :=
+by cases l; simp only [literal.flip, literal.eval, bnot_bnot]
 
-theorem eval_flip_of_eval {α : assignment} {l : literal} {b : bool} :
-  literal.eval α l = b → literal.eval α l.flip = !b :=
-assume h, by { rw eval_flip at h, exact congr_arg bnot h ▸ (bnot_bnot _).symm }
+theorem eval_flip_of_eval {α : assignment V} {l : literal V} {b : bool} :
+  l.eval α = b → l.flip.eval α = bnot b :=
+assume h, congr_arg bnot h ▸ eval_flip α l
 
-theorem eval_of_eval_flip {α : assignment} {l : literal} {b : bool} :
-  literal.eval α l.flip = b → literal.eval α l = !b :=
+theorem eval_of_eval_flip {α : assignment V} {l : literal V} {b : bool} :
+  literal.eval α l.flip = b → literal.eval α l = bnot b :=
+assume h, congr_arg bnot h ▸ eval_flip2 α l
+
+/-! # Positives and negatives -/
+
+protected def is_pos : literal V → Prop
+| (Pos _) := true
+| (Neg _) := false
+
+protected def is_neg : literal V → Prop
+| (Pos _) := false
+| (Neg _) := true
+
+-- Must be protected because of decidable.is_true
+protected def is_true (α : assignment V) (l : literal V) : Prop := 
+literal.eval α l = tt
+
+protected def is_false (α : assignment V) (l : literal V) : Prop :=
+literal.eval α l = ff
+
+-- is_pos, etc. are decidable
+instance : decidable_pred (literal.is_pos : literal V → Prop) :=
 begin
-  intro h,
-  rw eval_flip at h,
-  rw flip_flip l at h,
-  exact (bnot_bnot (literal.eval α l)) ▸ congr_arg bnot h,
+  intro l, cases l,
+  { unfold literal.is_pos, exact decidable.true },
+  { unfold literal.is_pos, exact decidable.false }
 end
 
-/-! # Miscellany -/
-
-def set_pos (l : literal) : literal := Pos (l.var)
-def set_neg (l : literal) : literal := Neg (l.var)
-
-def is_pos : literal → bool
-| (Pos _) := tt
-| (Neg _) := ff
-
-def is_neg : literal → bool
-| (Pos _) := ff
-| (Neg _) := tt
-
-@[simp] theorem pos_ne_neg (n : nat) : Pos n ≠ Neg n :=
-by simp
-
-theorem ne_of_ne_var {l₁ l₂ : literal} : l₁.var ≠ l₂.var → l₁ ≠ l₂ :=
+instance : decidable_pred (literal.is_neg : literal V → Prop) :=
 begin
-  contrapose,
-  simp,
-  intro h,
-  rw h
+  intro l, cases l,
+  { unfold literal.is_neg, exact decidable.false },
+  { unfold literal.is_neg, exact decidable.true }
 end
 
-theorem pos_or_neg_of_var_eq_nat {l : literal} {n : nat} : 
-  l.var = n → l = Pos n ∨ l = Neg n :=
-by cases l; simp [var]
+instance (α : assignment V) : decidable_pred (literal.is_true α) :=
+begin
+  intro l,
+  cases h : literal.eval α l;
+  { unfold literal.is_true, rw h, exact eq.decidable _ _ }
+end
+
+instance (α : assignment V) : decidable_pred (literal.is_false α) :=
+begin
+  intro l,
+  cases h : literal.eval α l;
+  { unfold literal.is_false, rw h, exact eq.decidable _ _ }
+end
+
+-- A literal can never be both positive and negative
+theorem is_pos_ne_is_neg (l : literal V) :
+  literal.is_pos l ≠ literal.is_neg l :=
+by cases l; simp [literal.is_pos, literal.is_neg]
+
+-- A literal can never be both true and false under the same assignment
+-- NOTE: A strange proof, can probably be simplified
+theorem is_true_ne_is_false (α : assignment V) :
+  (literal.is_true α) ≠ (literal.is_false α) :=
+begin
+  intro h,
+  have v := arbitrary (literal V),
+  have := congr_arg (λ (f : literal V → Prop), f v) h,
+  cases he : literal.eval α v;
+  { simp [literal.is_true, literal.is_false, he] at this, assumption }
+end
 
 end literal
