src/deprecated/literal.lean
@@ -1,0 +1,161 @@
+/-
+
+  This file contains the definition of a Boolean literal.
+  
+  Authors: Cayden Codel, Jeremy Avigad, Marijn Heule
+  Carnegie Mellon University
+
+-/
+
+import init.data.nat
+import init.logic
+import logic.function.basic
+import data.list.basic
+
+/- 
+  All propositional formulas are comprised of Boolean variables.
+  Here, we represent variables as natural numbers, which may then be evaluated
+  with an appropriate assignment of boolean values to those variables.
+
+  Literals are positive and negative instances of those variables.
+-/
+@[derive decidable_eq]
+inductive literal : Type
+| Pos : nat → literal
+| Neg : nat → literal
+
+/- Assignments give boolean values to the variables -/
+def assignment := nat → bool
+
+namespace literal
+
+open function
+
+/- Instance properties -/
+instance : inhabited literal := ⟨Pos 0⟩
+
+/- Extracts the natural number boolean variable of the literal -/
+def var : literal → nat
+| (Pos n) := n
+| (Neg n) := n
+
+/- Negated literals receive the opposite boolean value as the variable -/
+protected def eval (α : assignment) : literal → bool
+| (Pos n) := α n
+| (Neg n) := bnot (α n)
+
+/-! # Flip -/
+
+/- Flips the parity of the literal from positive to negative and vice versa -/
+def flip : literal → literal
+| (Pos n) := Neg n
+| (Neg n) := Pos n
+
+@[simp] theorem flip_ne (l : literal) : l.flip ≠ l :=
+by cases l; simp [flip]
+
+theorem flip_flip (l : literal) : l.flip.flip = l :=
+by cases l; simp only [flip]
+
+theorem flip_var_eq (l : literal) : l.flip.var = l.var :=
+by cases l; simp only [flip, var]
+
+@[simp] theorem flip_injective : injective (literal.flip) :=
+assume l₁ l₂ h, (flip_flip l₂) ▸ ((flip_flip l₁) ▸ (congr_arg flip h))
+
+theorem flip_inj {l₁ l₂ : literal} : l₁.flip = l₂.flip ↔ l₁ = l₂ :=
+flip_injective.eq_iff
+
+@[simp] theorem flip_surjective : surjective flip :=
+assume l, exists.intro l.flip (flip_flip l)
+
+@[simp] theorem flip_bijective : bijective flip :=
+⟨flip_injective, flip_surjective⟩
+
+lemma eq_or_flip_eq_of_var_eq {l₁ l₂ : literal} : 
+  l₁.var = l₂.var → l₁ = l₂ ∨ l₁.flip = l₂ :=
+by cases l₁; { cases l₂; simp [flip, var] }
+
+lemma var_eq_of_eq_or_flip_eq {l₁ l₂ : literal} : 
+  l₁ = l₂ ∨ l₁.flip = l₂ → l₁.var = l₂.var :=
+assume h, or.elim h
+  (assume : l₁ = l₂, congr_arg var this)
+  (assume : l₁.flip = l₂, congr_arg var this ▸ (flip_var_eq l₁).symm)
+
+theorem eq_or_flip_eq_iff_var_eq {l₁ l₂ : literal} : 
+  l₁.var = l₂.var ↔ l₁ = l₂ ∨ l₁.flip = l₂ :=
+⟨eq_or_flip_eq_of_var_eq, var_eq_of_eq_or_flip_eq⟩
+
+theorem flip_eq_iff_eq_flip {l₁ l₂ : literal} : l₁.flip = l₂ ↔ l₁ = l₂.flip :=
+⟨λ h, congr_arg flip h ▸ (flip_flip l₁).symm, λ h, (congr_arg flip h).symm ▸ flip_flip l₂⟩
+
+theorem flip_eq_of_ne_of_var_eq {l₁ l₂ : literal} :
+  l₁ ≠ l₂ → l₁.var = l₂.var → l₁.flip = l₂ :=
+begin
+  intros h₁ h₂,
+  cases eq_or_flip_eq_of_var_eq h₂,
+  { contradiction },
+  { exact h }
+end
+
+theorem eq_of_flip_ne_of_var_eq {l₁ l₂ : literal} :
+  l₁.flip ≠ l₂ → l₁.var = l₂.var → l₁ = l₂ :=
+begin
+  intros h₁ h₂,
+  cases eq_or_flip_eq_of_var_eq h₂,
+  { exact h },
+  { contradiction }
+end
+
+/-! # Flip evaluation -/
+
+theorem eval_flip (α : assignment) (l : literal) : 
+  literal.eval α l = bnot (literal.eval α l.flip) :=
+by cases l; simp only [flip, literal.eval, bnot_bnot]
+
+theorem eval_flip2 (α : assignment) (l : literal) : 
+  literal.eval α l.flip = bnot (literal.eval α l) :=
+by cases l; simp only [flip, literal.eval, bnot_bnot]
+
+theorem eval_flip_of_eval {α : assignment} {l : literal} {b : bool} :
+  literal.eval α l = b → literal.eval α l.flip = !b :=
+assume h, by { rw eval_flip at h, exact congr_arg bnot h ▸ (bnot_bnot _).symm }
+
+theorem eval_of_eval_flip {α : assignment} {l : literal} {b : bool} :
+  literal.eval α l.flip = b → literal.eval α l = !b :=
+begin
+  intro h,
+  rw eval_flip at h,
+  rw flip_flip l at h,
+  exact (bnot_bnot (literal.eval α l)) ▸ congr_arg bnot h,
+end
+
+/-! # Miscellany -/
+
+def set_pos (l : literal) : literal := Pos (l.var)
+def set_neg (l : literal) : literal := Neg (l.var)
+
+def is_pos : literal → bool
+| (Pos _) := tt
+| (Neg _) := ff
+
+def is_neg : literal → bool
+| (Pos _) := ff
+| (Neg _) := tt
+
+@[simp] theorem pos_ne_neg (n : nat) : Pos n ≠ Neg n :=
+by simp
+
+theorem ne_of_ne_var {l₁ l₂ : literal} : l₁.var ≠ l₂.var → l₁ ≠ l₂ :=
+begin
+  contrapose,
+  simp,
+  intro h,
+  rw h
+end
+
+theorem pos_or_neg_of_var_eq_nat {l : literal} {n : nat} : 
+  l.var = n → l = Pos n ∨ l = Neg n :=
+by cases l; simp [var]
+
+end literal
